revm: more definitions for revm_specification

CoqOfRust/revm/generate.py
@@ -7,7 +7,46 @@ sys.path.append(os.getcwd())
 import of_json
 
 
-def revm_bytecode_eof_header_types():
+def revm_bytecode_bytecode():
+    crate = "revm_bytecode"
+    top_level = json.load(open("revm/revm_bytecode/bytecode.json"))
+    output = of_json.get_header([
+        "Import revm.links.dependencies",
+    ])
+    output += "\n"
+    (prefix, ty_def) = of_json.find_top_level_item_by_name(crate, top_level, "Bytecode")
+    output += of_json.pp_type_enum(
+        prefix,
+        ty_def["TypeEnum"],
+    )
+    output += "\n"
+
+    with open("revm/revm_bytecode/links/bytecode.v", "w") as f:
+        f.write(output)
+
+
+def revm_bytecode_eof_body():
+    crate = "revm_bytecode"
+    top_level = json.load(open("revm/revm_bytecode/eof/body.json"))
+    output = of_json.get_header([
+        "alloc.links.alloc",
+        "alloc.links.vec",
+        "Import revm.links.dependencies",
+        "revm.revm_bytecode.eof.links.types_section",
+    ])
+    output += "\n"
+    (prefix, ty_def) = of_json.find_top_level_item_by_name(crate, top_level, "EofBody")
+    output += of_json.pp_type_struct_struct(
+        prefix,
+        ty_def["TypeStructStruct"],
+    )
+    output += "\n"
+
+    with open("revm/revm_bytecode/eof/links/body_Types.v", "w") as f:
+        f.write(output)
+
+
+def revm_bytecode_eof_header():
     crate = "revm_bytecode"
     top_level = json.load(open("revm/revm_bytecode/eof/header.json"))
     output = of_json.get_header([
@@ -27,7 +66,49 @@ def revm_bytecode_eof_header_types():
         f.write(output)
 
 
-def revm_interpreter_interpreter_action_eof_create_inputs_types():
+def revm_bytecode_eof_types_section():
+    crate = "revm_bytecode"
+    top_level = json.load(open("revm/revm_bytecode/eof/types_section.json"))
+    output = of_json.get_header([
+        "alloc.links.alloc",
+        "alloc.links.vec",
+        "Import revm.links.dependencies",
+    ])
+    output += "\n"
+    (prefix, ty_def) = of_json.find_top_level_item_by_name(crate, top_level, "TypesSection")
+    output += of_json.pp_type_struct_struct(
+        prefix,
+        ty_def["TypeStructStruct"],
+    )
+    output += "\n"
+
+    with open("revm/revm_bytecode/eof/links/types_section_Types.v", "w") as f:
+        f.write(output)
+
+
+def revm_bytecode_eof():
+    crate = "revm_bytecode"
+    top_level = json.load(open("revm/revm_bytecode/eof.json"))
+    output = of_json.get_header([
+        "alloc.links.alloc",
+        "alloc.links.vec",
+        "Import revm.links.dependencies",
+        "revm.revm_bytecode.eof.links.body",
+        "revm.revm_bytecode.eof.links.header",
+    ])
+    output += "\n"
+    (prefix, ty_def) = of_json.find_top_level_item_by_name(crate, top_level, "Eof")
+    output += of_json.pp_type_struct_struct(
+        prefix,
+        ty_def["TypeStructStruct"],
+    )
+    output += "\n"
+
+    with open("revm/revm_bytecode/links/eof_Types.v", "w") as f:
+        f.write(output)
+
+
+def revm_interpreter_interpreter_action_eof_create_inputs():
     crate = "revm_interpreter"
     top_level = json.load(open("revm/revm_interpreter/interpreter_action/eof_create_inputs.json"))
     output = of_json.get_header([
@@ -40,11 +121,73 @@ def revm_interpreter_interpreter_action_eof_create_inputs_types():
         prefix,
         ty_def["TypeEnum"],
     )
+    (prefix, ty_def) = of_json.find_top_level_item_by_name(crate, top_level, "EOFCreateInputs")
+    output += "\n\n"
+    output += of_json.pp_type_struct_struct(
+        prefix,
+        ty_def["TypeStructStruct"],
+    )
     output += "\n"
 
-    with open("revm/revm_interpreter/interpreter_action/links/eof_create_inputs_Types.v", "w") as f:
+    with open("revm/revm_interpreter/interpreter_action/links/eof_create_inputs.v", "w") as f:
         f.write(output)
 
 
-revm_bytecode_eof_header_types()
-revm_interpreter_interpreter_action_eof_create_inputs_types()
+# revm_bytecode_bytecode()
+# revm_bytecode_eof_body()
+# revm_bytecode_eof_header()
+# revm_bytecode_eof_types_section()
+# revm_bytecode_eof()
+# revm_interpreter_interpreter_action_eof_create_inputs()
+
+def get_all_type_definitions():
+    project_path = 'revm'
+    items = []
+    for crate in os.listdir(project_path):
+        crate_path = os.path.join(project_path, crate)
+
+        # Check if the crate is a directory
+        if os.path.isdir(crate_path):
+            print(f"Processing crate: {crate}")
+
+            # Loop through all files in the crate directory
+            for root, _, files in os.walk(crate_path):
+                for filename in files:
+                    # These files are too long and make an error in JSON parsing
+                    if filename == "opcode.json":
+                        continue
+                    # Check if the file has a .json extension
+                    if filename.endswith('.json'):
+                        file_path = os.path.join(root, filename)
+
+                        # Open and read the JSON file
+                        with open(file_path, 'r') as file:
+                            top_level = json.load(file)
+                            ty_defs = of_json.find_top_level_items_by_kind_in(
+                                crate,
+                                top_level,
+                                ["TypeStructStruct", "TypeEnum"],
+                            )
+                            if len(ty_defs) > 0:
+                                print(f"Found {len(ty_defs)} type definitions in {filename}")
+                                for (prefix, ty_def) in ty_defs:
+                                    print(f"  {prefix + [next(iter(ty_def.values()))['name']]}")
+                            items += ty_defs
+
+    # Pretty-print all the items
+    output = of_json.get_header([
+        "Import revm.links.dependencies",
+    ])
+    for (prefix, ty_def) in items:
+        print(f"Type definition: {prefix + [next(iter(ty_def.values()))['name']]}")
+        output += "\n"
+        if "TypeEnum" in ty_def:
+            output += of_json.pp_type_enum(prefix, ty_def["TypeEnum"])
+        elif "TypeStructStruct" in ty_def:
+            output += of_json.pp_type_struct_struct(prefix, ty_def["TypeStructStruct"])
+        output += "\n"
+
+    with open("revm/types.v", "w") as f:
+        f.write(output)
+
+get_all_type_definitions()
