CoqOfRust/revm/links/dependencies.v
@@ -1,12 +1,29 @@
 Require Import CoqOfRust.CoqOfRust.
 Require Import CoqOfRust.links.M.
 
+Module ruint.
+  Module Uint.
+    Parameter t : Z -> Z -> Set.
+
+    Parameter to_value : forall {BITS LIMBS : Z}, t BITS LIMBS -> Value.t.
+
+    Global Instance IsLink : forall {BITS LIMBS : Z}, Link (t BITS LIMBS) := {
+      Φ :=
+        Ty.apply
+          (Ty.path "ruint::Uint")
+          [ Value.Integer IntegerKind.Usize BITS; Value.Integer IntegerKind.Usize LIMBS ]
+          [];
+      φ := to_value;
+    }.
+  End Uint.
+End ruint.
+
 Module alloy_primitives.
   Module bits.
     Module links.
       Module address.
         Module Address.
-          Parameter t: Set.
+          Parameter t : Set.
 
           Parameter to_value : t -> Value.t.
 
@@ -35,17 +52,6 @@ Module alloy_primitives.
   End links.
 End alloy_primitives.
 
-Module Address.
-  Parameter t : Set.
-
-  Parameter to_value : t -> Value.t.
-
-  Global Instance IsLink : Link t := {
-    Φ := Ty.path "alloy_primitives::bits::address::Address";
-    φ := to_value;
-  }.
-End Address.
-
 Module FixedBytes.
   Parameter t : Set.
 
@@ -58,16 +64,8 @@ Module FixedBytes.
 End FixedBytes.
 
 Module U256.
-  Definition t : Set := Z.
-
-  Parameter to_value : t -> Value.t.
-
-  Definition size : Z := 256.
-
-  Global Instance IsLink : Link t := {
-    Φ := Ty.path "ruint::Uint";
-    φ := to_value;
-  }.
+  Definition t : Set :=
+    ruint.Uint.t 256 4.
 End U256.
 
 Module B256.
