CoqOfRust/revm/revm_bytecode/eof/links/body.v
@@ -1,0 +1,30 @@
+Require Import CoqOfRust.CoqOfRust.
+Require Import links.M.
+Require alloc.links.alloc.
+Require alloc.links.vec.
+Require Import revm.links.dependencies.
+Require revm.revm_bytecode.eof.links.types_section.
+
+Module EofBody.
+  Record t : Set := {
+    types_section: alloc.links.vec.Vec.t revm_bytecode.eof.links.types_section.TypesSection.t alloc.links.alloc.Global.t;
+    code_section: alloc.links.vec.Vec.t Usize.t alloc.links.alloc.Global.t;
+    code: alloy_primitives.links.bytes_.Bytes.t;
+    container_section: alloc.links.vec.Vec.t alloy_primitives.links.bytes_.Bytes.t alloc.links.alloc.Global.t;
+    data_section: alloy_primitives.links.bytes_.Bytes.t;
+    is_data_filled: bool;
+  }.
+
+  Global Instance IsLink : Link t := {
+    Φ := Ty.path "revm_bytecode::eof::body::EofBody";
+    φ '(Build_t types_section code_section code container_section data_section is_data_filled) :=
+      Value.StructRecord "revm_bytecode::eof::body::EofBody" [
+        ("types_section", φ types_section);
+        ("code_section", φ code_section);
+        ("code", φ code);
+        ("container_section", φ container_section);
+        ("data_section", φ data_section);
+        ("is_data_filled", φ is_data_filled)
+      ]
+  }.
+End EofBody.
