CoqOfRust/revm/revm_bytecode/eof/links/header.v
@@ -1,0 +1,28 @@
+Require Import CoqOfRust.CoqOfRust.
+Require Import links.M.
+Require alloc.links.alloc.
+Require alloc.links.vec.
+
+Module EofHeader.
+  Record t : Set := {
+    types_size: U16.t;
+    code_sizes: alloc.links.vec.Vec.t U16.t alloc.links.alloc.Global.t;
+    container_sizes: alloc.links.vec.Vec.t U16.t alloc.links.alloc.Global.t;
+    data_size: U16.t;
+    sum_code_sizes: Usize.t;
+    sum_container_sizes: Usize.t;
+  }.
+
+  Global Instance IsLink : Link t := {
+    Φ := Ty.path "revm_bytecode::eof::header::EofHeader";
+    φ '(Build_t types_size code_sizes container_sizes data_size sum_code_sizes sum_container_sizes) :=
+      Value.StructRecord "revm_bytecode::eof::header::EofHeader" [
+        ("types_size", φ types_size);
+        ("code_sizes", φ code_sizes);
+        ("container_sizes", φ container_sizes);
+        ("data_size", φ data_size);
+        ("sum_code_sizes", φ sum_code_sizes);
+        ("sum_container_sizes", φ sum_container_sizes)
+      ]
+  }.
+End EofHeader.
