CoqOfRust/revm/types.v
@@ -1,0 +1,2157 @@
+(* Generated file. Do not edit. *)
+Require Import CoqOfRust.CoqOfRust.
+Require Import links.M.
+Require Import revm.links.dependencies.
+
+Module InstructionTables.
+  Inductive t (W H CI: Set) : Set :=
+  | Plain
+    (_ : alloc.links.boxed.Box.t (array.t 256 (Function2.t (Ref.t Pointer.Kind.MutRef (revm_interpreter.links.interpreter.Interpreter.t W)) (Ref.t Pointer.Kind.MutRef H) ())) alloc.links.alloc.Global.t)
+  | Custom
+    (_ : alloc.links.boxed.Box.t (array.t 256 CI) alloc.links.alloc.Global.t)
+  .
+  Arguments Plain Custom {_ _ _}.
+
+  Global Instance IsLink (W H CI: Set) : Link t W H CI := {
+    Φ := Ty.path "revm_interpreter::table::InstructionTables";
+    φ x :=
+      match x with
+      | Plain γ0 =>
+        Value.StructTuple "revm_interpreter::table::InstructionTables::Plain" [
+          φ γ0
+        ]
+      | Custom γ0 =>
+        Value.StructTuple "revm_interpreter::table::InstructionTables::Custom" [
+          φ γ0
+        ]
+      end
+  }.
+End InstructionTables.
+
+Module Interpreter.
+  Record t {WIRE: Set} : Set := {
+    bytecode: Unknown type Associated;
+    stack: Unknown type Associated;
+    return_data: Unknown type Associated;
+    memory: Unknown type Associated;
+    input: Unknown type Associated;
+    sub_routine: Unknown type Associated;
+    control: Unknown type Associated;
+    runtime_flag: Unknown type Associated;
+    extend: Unknown type Associated;
+  }.
+  Arguments Build_t {_}.
+  Arguments t : clear implicits.
+
+  Global Instance IsLink {WIRE: Set} `{Link WIRE} : Link (t WIRE) := {
+    Φ := Ty.path "revm_interpreter::interpreter::Interpreter";
+    φ '(Build_t bytecode stack return_data memory input sub_routine control runtime_flag extend) :=
+      Value.StructRecord "revm_interpreter::interpreter::Interpreter" [
+        ("bytecode", φ bytecode);
+        ("stack", φ stack);
+        ("return_data", φ return_data);
+        ("memory", φ memory);
+        ("input", φ input);
+        ("sub_routine", φ sub_routine);
+        ("control", φ control);
+        ("runtime_flag", φ runtime_flag);
+        ("extend", φ extend)
+      ]
+  }.
+End Interpreter.
+
+Module EthInterpreter.
+  Record t {EXT MG: Set} : Set := {
+    _phantom: core.links.marker.PhantomData.t (Function0.t (EXT * MG));
+  }.
+  Arguments Build_t {_ _}.
+  Arguments t : clear implicits.
+
+  Global Instance IsLink {EXT MG: Set} `{Link EXT} `{Link MG} : Link (t EXT MG) := {
+    Φ := Ty.path "revm_interpreter::interpreter::EthInterpreter";
+    φ '(Build_t _phantom) :=
+      Value.StructRecord "revm_interpreter::interpreter::EthInterpreter" [
+        ("_phantom", φ _phantom)
+      ]
+  }.
+End EthInterpreter.
+
+Module EthInstructionProvider.
+  Record t {WIRE HOST: Set} : Set := {
+    instruction_table: alloc.links.rc.Rc.t (array.t 256 (Function2.t (Ref.t Pointer.Kind.MutRef (revm_interpreter.links.interpreter.Interpreter.t WIRE)) (Ref.t Pointer.Kind.MutRef HOST) ())) alloc.links.alloc.Global.t;
+  }.
+  Arguments Build_t {_ _}.
+  Arguments t : clear implicits.
+
+  Global Instance IsLink {WIRE HOST: Set} `{Link WIRE} `{Link HOST} : Link (t WIRE HOST) := {
+    Φ := Ty.path "revm_interpreter::interpreter::EthInstructionProvider";
+    φ '(Build_t instruction_table) :=
+      Value.StructRecord "revm_interpreter::interpreter::EthInstructionProvider" [
+        ("instruction_table", φ instruction_table)
+      ]
+  }.
+End EthInstructionProvider.
+
+Module InterpreterResult.
+  Record t : Set := {
+    result: revm_interpreter.links.instruction_result.InstructionResult.t;
+    output: alloy_primitives.links.bytes_.Bytes.t;
+    gas: revm_interpreter.links.gas.Gas.t;
+  }.
+
+  Global Instance IsLink : Link t := {
+    Φ := Ty.path "revm_interpreter::interpreter::InterpreterResult";
+    φ '(Build_t result output gas) :=
+      Value.StructRecord "revm_interpreter::interpreter::InterpreterResult" [
+        ("result", φ result);
+        ("output", φ output);
+        ("gas", φ gas)
+      ]
+  }.
+End InterpreterResult.
+
+Module FrameInput.
+  Inductive t : Set :=
+  | Call
+    (_ : alloc.links.boxed.Box.t revm_interpreter.interpreter_action.links.call_inputs.CallInputs.t alloc.links.alloc.Global.t)
+  | Create
+    (_ : alloc.links.boxed.Box.t revm_interpreter.interpreter_action.links.create_inputs.CreateInputs.t alloc.links.alloc.Global.t)
+  | EOFCreate
+    (_ : alloc.links.boxed.Box.t revm_interpreter.interpreter_action.links.eof_create_inputs.EOFCreateInputs.t alloc.links.alloc.Global.t)
+  .
+
+  Global Instance IsLink : Link t := {
+    Φ := Ty.path "revm_interpreter::interpreter_action::FrameInput";
+    φ x :=
+      match x with
+      | Call γ0 =>
+        Value.StructTuple "revm_interpreter::interpreter_action::FrameInput::Call" [
+          φ γ0
+        ]
+      | Create γ0 =>
+        Value.StructTuple "revm_interpreter::interpreter_action::FrameInput::Create" [
+          φ γ0
+        ]
+      | EOFCreate γ0 =>
+        Value.StructTuple "revm_interpreter::interpreter_action::FrameInput::EOFCreate" [
+          φ γ0
+        ]
+      end
+  }.
+End FrameInput.
+
+Module InterpreterAction.
+  Inductive t : Set :=
+  | NewFrame
+    (_ : revm_interpreter.links.interpreter_action.FrameInput.t)
+  | Return
+    (result : revm_interpreter.links.interpreter.InterpreterResult.t)
+  | None
+  .
+
+  Global Instance IsLink : Link t := {
+    Φ := Ty.path "revm_interpreter::interpreter_action::InterpreterAction";
+    φ x :=
+      match x with
+      | NewFrame γ0 =>
+        Value.StructTuple "revm_interpreter::interpreter_action::InterpreterAction::NewFrame" [
+          φ γ0
+        ]
+      | Return result =>
+        Value.StructRecord "revm_interpreter::interpreter_action::InterpreterAction::Return" [
+          ("result", φ result)
+        ]
+      | None  =>
+        Value.StructTuple "revm_interpreter::interpreter_action::InterpreterAction::None" []
+      end
+  }.
+End InterpreterAction.
+
+Module InstructionResult.
+  Inductive t : Set :=
+  | Continue
+  | Stop
+  | Return
+  | SelfDestruct
+  | ReturnContract
+  | Revert
+  | CallTooDeep
+  | OutOfFunds
+  | CreateInitCodeStartingEF00
+  | InvalidEOFInitCode
+  | InvalidExtDelegateCallTarget
+  | CallOrCreate
+  | OutOfGas
+  | MemoryOOG
+  | MemoryLimitOOG
+  | PrecompileOOG
+  | InvalidOperandOOG
+  | ReentrancySentryOOG
+  | OpcodeNotFound
+  | CallNotAllowedInsideStatic
+  | StateChangeDuringStaticCall
+  | InvalidFEOpcode
+  | InvalidJump
+  | NotActivated
+  | StackUnderflow
+  | StackOverflow
+  | OutOfOffset
+  | CreateCollision
+  | OverflowPayment
+  | PrecompileError
+  | NonceOverflow
+  | CreateContractSizeLimit
+  | CreateContractStartingWithEF
+  | CreateInitCodeSizeLimit
+  | FatalExternalError
+  | ReturnContractInNotInitEOF
+  | EOFOpcodeDisabledInLegacy
+  | SubRoutineStackOverflow
+  | EofAuxDataOverflow
+  | EofAuxDataTooSmall
+  | InvalidEXTCALLTarget
+  .
+
+  Global Instance IsLink : Link t := {
+    Φ := Ty.path "revm_interpreter::instruction_result::InstructionResult";
+    φ x :=
+      match x with
+      | Continue  =>
+        Value.StructTuple "revm_interpreter::instruction_result::InstructionResult::Continue" []
+      | Stop  =>
+        Value.StructTuple "revm_interpreter::instruction_result::InstructionResult::Stop" []
+      | Return  =>
+        Value.StructTuple "revm_interpreter::instruction_result::InstructionResult::Return" []
+      | SelfDestruct  =>
+        Value.StructTuple "revm_interpreter::instruction_result::InstructionResult::SelfDestruct" []
+      | ReturnContract  =>
+        Value.StructTuple "revm_interpreter::instruction_result::InstructionResult::ReturnContract" []
+      | Revert  =>
+        Value.StructTuple "revm_interpreter::instruction_result::InstructionResult::Revert" []
+      | CallTooDeep  =>
+        Value.StructTuple "revm_interpreter::instruction_result::InstructionResult::CallTooDeep" []
+      | OutOfFunds  =>
+        Value.StructTuple "revm_interpreter::instruction_result::InstructionResult::OutOfFunds" []
+      | CreateInitCodeStartingEF00  =>
+        Value.StructTuple "revm_interpreter::instruction_result::InstructionResult::CreateInitCodeStartingEF00" []
+      | InvalidEOFInitCode  =>
+        Value.StructTuple "revm_interpreter::instruction_result::InstructionResult::InvalidEOFInitCode" []
+      | InvalidExtDelegateCallTarget  =>
+        Value.StructTuple "revm_interpreter::instruction_result::InstructionResult::InvalidExtDelegateCallTarget" []
+      | CallOrCreate  =>
+        Value.StructTuple "revm_interpreter::instruction_result::InstructionResult::CallOrCreate" []
+      | OutOfGas  =>
+        Value.StructTuple "revm_interpreter::instruction_result::InstructionResult::OutOfGas" []
+      | MemoryOOG  =>
+        Value.StructTuple "revm_interpreter::instruction_result::InstructionResult::MemoryOOG" []
+      | MemoryLimitOOG  =>
+        Value.StructTuple "revm_interpreter::instruction_result::InstructionResult::MemoryLimitOOG" []
+      | PrecompileOOG  =>
+        Value.StructTuple "revm_interpreter::instruction_result::InstructionResult::PrecompileOOG" []
+      | InvalidOperandOOG  =>
+        Value.StructTuple "revm_interpreter::instruction_result::InstructionResult::InvalidOperandOOG" []
+      | ReentrancySentryOOG  =>
+        Value.StructTuple "revm_interpreter::instruction_result::InstructionResult::ReentrancySentryOOG" []
+      | OpcodeNotFound  =>
+        Value.StructTuple "revm_interpreter::instruction_result::InstructionResult::OpcodeNotFound" []
+      | CallNotAllowedInsideStatic  =>
+        Value.StructTuple "revm_interpreter::instruction_result::InstructionResult::CallNotAllowedInsideStatic" []
+      | StateChangeDuringStaticCall  =>
+        Value.StructTuple "revm_interpreter::instruction_result::InstructionResult::StateChangeDuringStaticCall" []
+      | InvalidFEOpcode  =>
+        Value.StructTuple "revm_interpreter::instruction_result::InstructionResult::InvalidFEOpcode" []
+      | InvalidJump  =>
+        Value.StructTuple "revm_interpreter::instruction_result::InstructionResult::InvalidJump" []
+      | NotActivated  =>
+        Value.StructTuple "revm_interpreter::instruction_result::InstructionResult::NotActivated" []
+      | StackUnderflow  =>
+        Value.StructTuple "revm_interpreter::instruction_result::InstructionResult::StackUnderflow" []
+      | StackOverflow  =>
+        Value.StructTuple "revm_interpreter::instruction_result::InstructionResult::StackOverflow" []
+      | OutOfOffset  =>
+        Value.StructTuple "revm_interpreter::instruction_result::InstructionResult::OutOfOffset" []
+      | CreateCollision  =>
+        Value.StructTuple "revm_interpreter::instruction_result::InstructionResult::CreateCollision" []
+      | OverflowPayment  =>
+        Value.StructTuple "revm_interpreter::instruction_result::InstructionResult::OverflowPayment" []
+      | PrecompileError  =>
+        Value.StructTuple "revm_interpreter::instruction_result::InstructionResult::PrecompileError" []
+      | NonceOverflow  =>
+        Value.StructTuple "revm_interpreter::instruction_result::InstructionResult::NonceOverflow" []
+      | CreateContractSizeLimit  =>
+        Value.StructTuple "revm_interpreter::instruction_result::InstructionResult::CreateContractSizeLimit" []
+      | CreateContractStartingWithEF  =>
+        Value.StructTuple "revm_interpreter::instruction_result::InstructionResult::CreateContractStartingWithEF" []
+      | CreateInitCodeSizeLimit  =>
+        Value.StructTuple "revm_interpreter::instruction_result::InstructionResult::CreateInitCodeSizeLimit" []
+      | FatalExternalError  =>
+        Value.StructTuple "revm_interpreter::instruction_result::InstructionResult::FatalExternalError" []
+      | ReturnContractInNotInitEOF  =>
+        Value.StructTuple "revm_interpreter::instruction_result::InstructionResult::ReturnContractInNotInitEOF" []
+      | EOFOpcodeDisabledInLegacy  =>
+        Value.StructTuple "revm_interpreter::instruction_result::InstructionResult::EOFOpcodeDisabledInLegacy" []
+      | SubRoutineStackOverflow  =>
+        Value.StructTuple "revm_interpreter::instruction_result::InstructionResult::SubRoutineStackOverflow" []
+      | EofAuxDataOverflow  =>
+        Value.StructTuple "revm_interpreter::instruction_result::InstructionResult::EofAuxDataOverflow" []
+      | EofAuxDataTooSmall  =>
+        Value.StructTuple "revm_interpreter::instruction_result::InstructionResult::EofAuxDataTooSmall" []
+      | InvalidEXTCALLTarget  =>
+        Value.StructTuple "revm_interpreter::instruction_result::InstructionResult::InvalidEXTCALLTarget" []
+      end
+  }.
+End InstructionResult.
+
+Module InternalResult.
+  Inductive t : Set :=
+  | InternalContinue
+  | InternalCallOrCreate
+  | CreateInitCodeStartingEF00
+  | InvalidExtDelegateCallTarget
+  .
+
+  Global Instance IsLink : Link t := {
+    Φ := Ty.path "revm_interpreter::instruction_result::InternalResult";
+    φ x :=
+      match x with
+      | InternalContinue  =>
+        Value.StructTuple "revm_interpreter::instruction_result::InternalResult::InternalContinue" []
+      | InternalCallOrCreate  =>
+        Value.StructTuple "revm_interpreter::instruction_result::InternalResult::InternalCallOrCreate" []
+      | CreateInitCodeStartingEF00  =>
+        Value.StructTuple "revm_interpreter::instruction_result::InternalResult::CreateInitCodeStartingEF00" []
+      | InvalidExtDelegateCallTarget  =>
+        Value.StructTuple "revm_interpreter::instruction_result::InternalResult::InvalidExtDelegateCallTarget" []
+      end
+  }.
+End InternalResult.
+
+Module SuccessOrHalt.
+  Inductive t (HaltReasonT: Set) : Set :=
+  | Success
+    (_ : revm_context_interface.links.result.SuccessReason.t)
+  | Revert
+  | Halt
+    (_ : HaltReasonT)
+  | FatalExternalError
+  | Internal
+    (_ : revm_interpreter.links.instruction_result.InternalResult.t)
+  .
+  Arguments Success Revert Halt FatalExternalError Internal {_}.
+
+  Global Instance IsLink (HaltReasonT: Set) : Link t HaltReasonT := {
+    Φ := Ty.path "revm_interpreter::instruction_result::SuccessOrHalt";
+    φ x :=
+      match x with
+      | Success γ0 =>
+        Value.StructTuple "revm_interpreter::instruction_result::SuccessOrHalt::Success" [
+          φ γ0
+        ]
+      | Revert  =>
+        Value.StructTuple "revm_interpreter::instruction_result::SuccessOrHalt::Revert" []
+      | Halt γ0 =>
+        Value.StructTuple "revm_interpreter::instruction_result::SuccessOrHalt::Halt" [
+          φ γ0
+        ]
+      | FatalExternalError  =>
+        Value.StructTuple "revm_interpreter::instruction_result::SuccessOrHalt::FatalExternalError" []
+      | Internal γ0 =>
+        Value.StructTuple "revm_interpreter::instruction_result::SuccessOrHalt::Internal" [
+          φ γ0
+        ]
+      end
+  }.
+End SuccessOrHalt.
+
+Module Gas.
+  Record t : Set := {
+    limit: U64.t;
+    remaining: U64.t;
+    refunded: I64.t;
+    memory: revm_interpreter.links.gas.MemoryGas.t;
+  }.
+
+  Global Instance IsLink : Link t := {
+    Φ := Ty.path "revm_interpreter::gas::Gas";
+    φ '(Build_t limit remaining refunded memory) :=
+      Value.StructRecord "revm_interpreter::gas::Gas" [
+        ("limit", φ limit);
+        ("remaining", φ remaining);
+        ("refunded", φ refunded);
+        ("memory", φ memory)
+      ]
+  }.
+End Gas.
+
+Module MemoryExtensionResult.
+  Inductive t : Set :=
+  | Extended
+  | Same
+  | OutOfGas
+  .
+
+  Global Instance IsLink : Link t := {
+    Φ := Ty.path "revm_interpreter::gas::MemoryExtensionResult";
+    φ x :=
+      match x with
+      | Extended  =>
+        Value.StructTuple "revm_interpreter::gas::MemoryExtensionResult::Extended" []
+      | Same  =>
+        Value.StructTuple "revm_interpreter::gas::MemoryExtensionResult::Same" []
+      | OutOfGas  =>
+        Value.StructTuple "revm_interpreter::gas::MemoryExtensionResult::OutOfGas" []
+      end
+  }.
+End MemoryExtensionResult.
+
+Module MemoryGas.
+  Record t : Set := {
+    words_num: Usize.t;
+    expansion_cost: U64.t;
+  }.
+
+  Global Instance IsLink : Link t := {
+    Φ := Ty.path "revm_interpreter::gas::MemoryGas";
+    φ '(Build_t words_num expansion_cost) :=
+      Value.StructRecord "revm_interpreter::gas::MemoryGas" [
+        ("words_num", φ words_num);
+        ("expansion_cost", φ expansion_cost)
+      ]
+  }.
+End MemoryGas.
+
+Module InputsImpl.
+  Record t : Set := {
+    target_address: alloy_primitives.bits.links.address.Address.t;
+    caller_address: alloy_primitives.bits.links.address.Address.t;
+    input: alloy_primitives.links.bytes_.Bytes.t;
+    call_value: ruint.Uint.t 256 4;
+  }.
+
+  Global Instance IsLink : Link t := {
+    Φ := Ty.path "revm_interpreter::interpreter::input::InputsImpl";
+    φ '(Build_t target_address caller_address input call_value) :=
+      Value.StructRecord "revm_interpreter::interpreter::input::InputsImpl" [
+        ("target_address", φ target_address);
+        ("caller_address", φ caller_address);
+        ("input", φ input);
+        ("call_value", φ call_value)
+      ]
+  }.
+End InputsImpl.
+
+Module SharedMemory.
+  Record t : Set := {
+    buffer: alloc.links.vec.Vec.t U8.t alloc.links.alloc.Global.t;
+    checkpoints: alloc.links.vec.Vec.t Usize.t alloc.links.alloc.Global.t;
+    last_checkpoint: Usize.t;
+  }.
+
+  Global Instance IsLink : Link t := {
+    Φ := Ty.path "revm_interpreter::interpreter::shared_memory::SharedMemory";
+    φ '(Build_t buffer checkpoints last_checkpoint) :=
+      Value.StructRecord "revm_interpreter::interpreter::shared_memory::SharedMemory" [
+        ("buffer", φ buffer);
+        ("checkpoints", φ checkpoints);
+        ("last_checkpoint", φ last_checkpoint)
+      ]
+  }.
+End SharedMemory.
+
+Module LoopControl.
+  Record t : Set := {
+    instruction_result: revm_interpreter.links.instruction_result.InstructionResult.t;
+    next_action: revm_interpreter.links.interpreter_action.InterpreterAction.t;
+    gas: revm_interpreter.links.gas.Gas.t;
+  }.
+
+  Global Instance IsLink : Link t := {
+    Φ := Ty.path "revm_interpreter::interpreter::loop_control::LoopControl";
+    φ '(Build_t instruction_result next_action gas) :=
+      Value.StructRecord "revm_interpreter::interpreter::loop_control::LoopControl" [
+        ("instruction_result", φ instruction_result);
+        ("next_action", φ next_action);
+        ("gas", φ gas)
+      ]
+  }.
+End LoopControl.
+
+Module Stack.
+  Record t : Set := {
+    data: alloc.links.vec.Vec.t (ruint.Uint.t 256 4) alloc.links.alloc.Global.t;
+  }.
+
+  Global Instance IsLink : Link t := {
+    Φ := Ty.path "revm_interpreter::interpreter::stack::Stack";
+    φ '(Build_t data) :=
+      Value.StructRecord "revm_interpreter::interpreter::stack::Stack" [
+        ("data", φ data)
+      ]
+  }.
+End Stack.
+
+Module ExtBytecode.
+  Record t : Set := {
+    base: revm_bytecode.links.bytecode.Bytecode.t;
+    instruction_pointer: Ref.t Pointer.Kind.ConstPointer U8.t;
+  }.
+
+  Global Instance IsLink : Link t := {
+    Φ := Ty.path "revm_interpreter::interpreter::ext_bytecode::ExtBytecode";
+    φ '(Build_t base instruction_pointer) :=
+      Value.StructRecord "revm_interpreter::interpreter::ext_bytecode::ExtBytecode" [
+        ("base", φ base);
+        ("instruction_pointer", φ instruction_pointer)
+      ]
+  }.
+End ExtBytecode.
+
+Module RuntimeFlags.
+  Record t : Set := {
+    is_static: bool;
+    is_eof_init: bool;
+    is_eof: bool;
+    spec_id: revm_specification.links.hardfork.SpecId.t;
+  }.
+
+  Global Instance IsLink : Link t := {
+    Φ := Ty.path "revm_interpreter::interpreter::runtime_flags::RuntimeFlags";
+    φ '(Build_t is_static is_eof_init is_eof spec_id) :=
+      Value.StructRecord "revm_interpreter::interpreter::runtime_flags::RuntimeFlags" [
+        ("is_static", φ is_static);
+        ("is_eof_init", φ is_eof_init);
+        ("is_eof", φ is_eof);
+        ("spec_id", φ spec_id)
+      ]
+  }.
+End RuntimeFlags.
+
+Module SubRoutineReturnFrame.
+  Record t : Set := {
+    idx: Usize.t;
+    pc: Usize.t;
+  }.
+
+  Global Instance IsLink : Link t := {
+    Φ := Ty.path "revm_interpreter::interpreter::subroutine_stack::SubRoutineReturnFrame";
+    φ '(Build_t idx pc) :=
+      Value.StructRecord "revm_interpreter::interpreter::subroutine_stack::SubRoutineReturnFrame" [
+        ("idx", φ idx);
+        ("pc", φ pc)
+      ]
+  }.
+End SubRoutineReturnFrame.
+
+Module SubRoutineImpl.
+  Record t : Set := {
+    return_stack: alloc.links.vec.Vec.t revm_interpreter.interpreter.links.subroutine_stack.SubRoutineReturnFrame.t alloc.links.alloc.Global.t;
+    current_code_idx: Usize.t;
+  }.
+
+  Global Instance IsLink : Link t := {
+    Φ := Ty.path "revm_interpreter::interpreter::subroutine_stack::SubRoutineImpl";
+    φ '(Build_t return_stack current_code_idx) :=
+      Value.StructRecord "revm_interpreter::interpreter::subroutine_stack::SubRoutineImpl" [
+        ("return_stack", φ return_stack);
+        ("current_code_idx", φ current_code_idx)
+      ]
+  }.
+End SubRoutineImpl.
+
+Module Sign.
+  Inductive t : Set :=
+  | Minus
+  | Zero
+  | Plus
+  .
+
+  Global Instance IsLink : Link t := {
+    Φ := Ty.path "revm_interpreter::instructions::i256::Sign";
+    φ x :=
+      match x with
+      | Minus  =>
+        Value.StructTuple "revm_interpreter::instructions::i256::Sign::Minus" []
+      | Zero  =>
+        Value.StructTuple "revm_interpreter::instructions::i256::Sign::Zero" []
+      | Plus  =>
+        Value.StructTuple "revm_interpreter::instructions::i256::Sign::Plus" []
+      end
+  }.
+End Sign.
+
+Module CallInputs.
+  Record t : Set := {
+    input: alloy_primitives.links.bytes_.Bytes.t;
+    return_memory_offset: core.ops.links.range.Range.t Usize.t;
+    gas_limit: U64.t;
+    bytecode_address: alloy_primitives.bits.links.address.Address.t;
+    target_address: alloy_primitives.bits.links.address.Address.t;
+    caller: alloy_primitives.bits.links.address.Address.t;
+    value: revm_interpreter.interpreter_action.links.call_inputs.CallValue.t;
+    scheme: revm_interpreter.interpreter_action.links.call_inputs.CallScheme.t;
+    is_static: bool;
+    is_eof: bool;
+  }.
+
+  Global Instance IsLink : Link t := {
+    Φ := Ty.path "revm_interpreter::interpreter_action::call_inputs::CallInputs";
+    φ '(Build_t input return_memory_offset gas_limit bytecode_address target_address caller value scheme is_static is_eof) :=
+      Value.StructRecord "revm_interpreter::interpreter_action::call_inputs::CallInputs" [
+        ("input", φ input);
+        ("return_memory_offset", φ return_memory_offset);
+        ("gas_limit", φ gas_limit);
+        ("bytecode_address", φ bytecode_address);
+        ("target_address", φ target_address);
+        ("caller", φ caller);
+        ("value", φ value);
+        ("scheme", φ scheme);
+        ("is_static", φ is_static);
+        ("is_eof", φ is_eof)
+      ]
+  }.
+End CallInputs.
+
+Module CallScheme.
+  Inductive t : Set :=
+  | Call
+  | CallCode
+  | DelegateCall
+  | StaticCall
+  | ExtCall
+  | ExtStaticCall
+  | ExtDelegateCall
+  .
+
+  Global Instance IsLink : Link t := {
+    Φ := Ty.path "revm_interpreter::interpreter_action::call_inputs::CallScheme";
+    φ x :=
+      match x with
+      | Call  =>
+        Value.StructTuple "revm_interpreter::interpreter_action::call_inputs::CallScheme::Call" []
+      | CallCode  =>
+        Value.StructTuple "revm_interpreter::interpreter_action::call_inputs::CallScheme::CallCode" []
+      | DelegateCall  =>
+        Value.StructTuple "revm_interpreter::interpreter_action::call_inputs::CallScheme::DelegateCall" []
+      | StaticCall  =>
+        Value.StructTuple "revm_interpreter::interpreter_action::call_inputs::CallScheme::StaticCall" []
+      | ExtCall  =>
+        Value.StructTuple "revm_interpreter::interpreter_action::call_inputs::CallScheme::ExtCall" []
+      | ExtStaticCall  =>
+        Value.StructTuple "revm_interpreter::interpreter_action::call_inputs::CallScheme::ExtStaticCall" []
+      | ExtDelegateCall  =>
+        Value.StructTuple "revm_interpreter::interpreter_action::call_inputs::CallScheme::ExtDelegateCall" []
+      end
+  }.
+End CallScheme.
+
+Module CallValue.
+  Inductive t : Set :=
+  | Transfer
+    (_ : ruint.Uint.t 256 4)
+  | Apparent
+    (_ : ruint.Uint.t 256 4)
+  .
+
+  Global Instance IsLink : Link t := {
+    Φ := Ty.path "revm_interpreter::interpreter_action::call_inputs::CallValue";
+    φ x :=
+      match x with
+      | Transfer γ0 =>
+        Value.StructTuple "revm_interpreter::interpreter_action::call_inputs::CallValue::Transfer" [
+          φ γ0
+        ]
+      | Apparent γ0 =>
+        Value.StructTuple "revm_interpreter::interpreter_action::call_inputs::CallValue::Apparent" [
+          φ γ0
+        ]
+      end
+  }.
+End CallValue.
+
+Module EOFCreateKind.
+  Inductive t : Set :=
+  | Tx
+    (initdata : alloy_primitives.links.bytes_.Bytes.t)
+  | Opcode
+    (initcode : revm_bytecode.links.eof.Eof.t)
+    (input : alloy_primitives.links.bytes_.Bytes.t)
+    (created_address : alloy_primitives.bits.links.address.Address.t)
+  .
+
+  Global Instance IsLink : Link t := {
+    Φ := Ty.path "revm_interpreter::interpreter_action::eof_create_inputs::EOFCreateKind";
+    φ x :=
+      match x with
+      | Tx initdata =>
+        Value.StructRecord "revm_interpreter::interpreter_action::eof_create_inputs::EOFCreateKind::Tx" [
+          ("initdata", φ initdata)
+        ]
+      | Opcode initcode input created_address =>
+        Value.StructRecord "revm_interpreter::interpreter_action::eof_create_inputs::EOFCreateKind::Opcode" [
+          ("initcode", φ initcode);
+          ("input", φ input);
+          ("created_address", φ created_address)
+        ]
+      end
+  }.
+End EOFCreateKind.
+
+Module EOFCreateInputs.
+  Record t : Set := {
+    caller: alloy_primitives.bits.links.address.Address.t;
+    value: ruint.Uint.t 256 4;
+    gas_limit: U64.t;
+    kind: revm_interpreter.interpreter_action.links.eof_create_inputs.EOFCreateKind.t;
+  }.
+
+  Global Instance IsLink : Link t := {
+    Φ := Ty.path "revm_interpreter::interpreter_action::eof_create_inputs::EOFCreateInputs";
+    φ '(Build_t caller value gas_limit kind) :=
+      Value.StructRecord "revm_interpreter::interpreter_action::eof_create_inputs::EOFCreateInputs" [
+        ("caller", φ caller);
+        ("value", φ value);
+        ("gas_limit", φ gas_limit);
+        ("kind", φ kind)
+      ]
+  }.
+End EOFCreateInputs.
+
+Module CreateInputs.
+  Record t : Set := {
+    caller: alloy_primitives.bits.links.address.Address.t;
+    scheme: revm_context_interface.links.cfg.CreateScheme.t;
+    value: ruint.Uint.t 256 4;
+    init_code: alloy_primitives.links.bytes_.Bytes.t;
+    gas_limit: U64.t;
+  }.
+
+  Global Instance IsLink : Link t := {
+    Φ := Ty.path "revm_interpreter::interpreter_action::create_inputs::CreateInputs";
+    φ '(Build_t caller scheme value init_code gas_limit) :=
+      Value.StructRecord "revm_interpreter::interpreter_action::create_inputs::CreateInputs" [
+        ("caller", φ caller);
+        ("scheme", φ scheme);
+        ("value", φ value);
+        ("init_code", φ init_code);
+        ("gas_limit", φ gas_limit)
+      ]
+  }.
+End CreateInputs.
+
+Module CallOutcome.
+  Record t : Set := {
+    result: revm_interpreter.links.interpreter.InterpreterResult.t;
+    memory_offset: core.ops.links.range.Range.t Usize.t;
+  }.
+
+  Global Instance IsLink : Link t := {
+    Φ := Ty.path "revm_interpreter::interpreter_action::call_outcome::CallOutcome";
+    φ '(Build_t result memory_offset) :=
+      Value.StructRecord "revm_interpreter::interpreter_action::call_outcome::CallOutcome" [
+        ("result", φ result);
+        ("memory_offset", φ memory_offset)
+      ]
+  }.
+End CallOutcome.
+
+Module CreateOutcome.
+  Record t : Set := {
+    result: revm_interpreter.links.interpreter.InterpreterResult.t;
+    address: core.links.option.Option.t alloy_primitives.bits.links.address.Address.t;
+  }.
+
+  Global Instance IsLink : Link t := {
+    Φ := Ty.path "revm_interpreter::interpreter_action::create_outcome::CreateOutcome";
+    φ '(Build_t result address) :=
+      Value.StructRecord "revm_interpreter::interpreter_action::create_outcome::CreateOutcome" [
+        ("result", φ result);
+        ("address", φ address)
+      ]
+  }.
+End CreateOutcome.
+
+Module AnalysisKind.
+  Inductive t : Set :=
+  | Raw
+  | Analyse
+  .
+
+  Global Instance IsLink : Link t := {
+    Φ := Ty.path "revm_context_interface::cfg::AnalysisKind";
+    φ x :=
+      match x with
+      | Raw  =>
+        Value.StructTuple "revm_context_interface::cfg::AnalysisKind::Raw" []
+      | Analyse  =>
+        Value.StructTuple "revm_context_interface::cfg::AnalysisKind::Analyse" []
+      end
+  }.
+End AnalysisKind.
+
+Module CreateScheme.
+  Inductive t : Set :=
+  | Create
+  | Create2
+    (salt : ruint.Uint.t 256 4)
+  .
+
+  Global Instance IsLink : Link t := {
+    Φ := Ty.path "revm_context_interface::cfg::CreateScheme";
+    φ x :=
+      match x with
+      | Create  =>
+        Value.StructTuple "revm_context_interface::cfg::CreateScheme::Create" []
+      | Create2 salt =>
+        Value.StructRecord "revm_context_interface::cfg::CreateScheme::Create2" [
+          ("salt", φ salt)
+        ]
+      end
+  }.
+End CreateScheme.
+
+Module ResultAndState.
+  Record t {HaltReasonT: Set} : Set := {
+    result: revm_context_interface.links.result.ExecutionResult.t HaltReasonT;
+    state: hashbrown.links.map.HashMap.t alloy_primitives.bits.links.address.Address.t revm_state.Account.t foldhash.seed.links.fast.RandomState.t hashbrown.raw.alloc.links.inner.Global.t;
+  }.
+  Arguments Build_t {_}.
+  Arguments t : clear implicits.
+
+  Global Instance IsLink {HaltReasonT: Set} `{Link HaltReasonT} : Link (t HaltReasonT) := {
+    Φ := Ty.path "revm_context_interface::result::ResultAndState";
+    φ '(Build_t result state) :=
+      Value.StructRecord "revm_context_interface::result::ResultAndState" [
+        ("result", φ result);
+        ("state", φ state)
+      ]
+  }.
+End ResultAndState.
+
+Module ExecutionResult.
+  Inductive t (HaltReasonT: Set) : Set :=
+  | Success
+    (reason : revm_context_interface.links.result.SuccessReason.t)
+    (gas_used : U64.t)
+    (gas_refunded : U64.t)
+    (logs : alloc.links.vec.Vec.t (alloy_primitives.links.log.Log.t alloy_primitives.links.log.LogData.t) alloc.links.alloc.Global.t)
+    (output : revm_context_interface.links.result.Output.t)
+  | Revert
+    (gas_used : U64.t)
+    (output : alloy_primitives.links.bytes_.Bytes.t)
+  | Halt
+    (reason : HaltReasonT)
+    (gas_used : U64.t)
+  .
+  Arguments Success Revert Halt {_}.
+
+  Global Instance IsLink (HaltReasonT: Set) : Link t HaltReasonT := {
+    Φ := Ty.path "revm_context_interface::result::ExecutionResult";
+    φ x :=
+      match x with
+      | Success reason gas_used gas_refunded logs output =>
+        Value.StructRecord "revm_context_interface::result::ExecutionResult::Success" [
+          ("reason", φ reason);
+          ("gas_used", φ gas_used);
+          ("gas_refunded", φ gas_refunded);
+          ("logs", φ logs);
+          ("output", φ output)
+        ]
+      | Revert gas_used output =>
+        Value.StructRecord "revm_context_interface::result::ExecutionResult::Revert" [
+          ("gas_used", φ gas_used);
+          ("output", φ output)
+        ]
+      | Halt reason gas_used =>
+        Value.StructRecord "revm_context_interface::result::ExecutionResult::Halt" [
+          ("reason", φ reason);
+          ("gas_used", φ gas_used)
+        ]
+      end
+  }.
+End ExecutionResult.
+
+Module Output.
+  Inductive t : Set :=
+  | Call
+    (_ : alloy_primitives.links.bytes_.Bytes.t)
+  | Create
+    (_ : alloy_primitives.links.bytes_.Bytes.t)
+    (_ : core.links.option.Option.t alloy_primitives.bits.links.address.Address.t)
+  .
+
+  Global Instance IsLink : Link t := {
+    Φ := Ty.path "revm_context_interface::result::Output";
+    φ x :=
+      match x with
+      | Call γ0 =>
+        Value.StructTuple "revm_context_interface::result::Output::Call" [
+          φ γ0
+        ]
+      | Create γ0 γ1 =>
+        Value.StructTuple "revm_context_interface::result::Output::Create" [
+          φ γ0;
+          φ γ1
+        ]
+      end
+  }.
+End Output.
+
+Module EVMError.
+  Inductive t (DBError TransactionError: Set) : Set :=
+  | Transaction
+    (_ : TransactionError)
+  | Header
+    (_ : revm_context_interface.links.result.InvalidHeader.t)
+  | Database
+    (_ : DBError)
+  | Custom
+    (_ : alloc.links.string.String.t)
+  | Precompile
+    (_ : alloc.links.string.String.t)
+  .
+  Arguments Transaction Header Database Custom Precompile {_ _}.
+
+  Global Instance IsLink (DBError TransactionError: Set) : Link t DBError TransactionError := {
+    Φ := Ty.path "revm_context_interface::result::EVMError";
+    φ x :=
+      match x with
+      | Transaction γ0 =>
+        Value.StructTuple "revm_context_interface::result::EVMError::Transaction" [
+          φ γ0
+        ]
+      | Header γ0 =>
+        Value.StructTuple "revm_context_interface::result::EVMError::Header" [
+          φ γ0
+        ]
+      | Database γ0 =>
+        Value.StructTuple "revm_context_interface::result::EVMError::Database" [
+          φ γ0
+        ]
+      | Custom γ0 =>
+        Value.StructTuple "revm_context_interface::result::EVMError::Custom" [
+          φ γ0
+        ]
+      | Precompile γ0 =>
+        Value.StructTuple "revm_context_interface::result::EVMError::Precompile" [
+          φ γ0
+        ]
+      end
+  }.
+End EVMError.
+
+Module InvalidTransaction.
+  Inductive t : Set :=
+  | PriorityFeeGreaterThanMaxFee
+  | GasPriceLessThanBasefee
+  | CallerGasLimitMoreThanBlock
+  | CallGasCostMoreThanGasLimit
+  | RejectCallerWithCode
+  | LackOfFundForMaxFee
+    (fee : alloc.links.boxed.Box.t (ruint.Uint.t 256 4) alloc.links.alloc.Global.t)
+    (balance : alloc.links.boxed.Box.t (ruint.Uint.t 256 4) alloc.links.alloc.Global.t)
+  | OverflowPaymentInTransaction
+  | NonceOverflowInTransaction
+  | NonceTooHigh
+    (tx : U64.t)
+    (state : U64.t)
+  | NonceTooLow
+    (tx : U64.t)
+    (state : U64.t)
+  | CreateInitCodeSizeLimit
+  | InvalidChainId
+  | AccessListNotSupported
+  | MaxFeePerBlobGasNotSupported
+  | BlobVersionedHashesNotSupported
+  | BlobGasPriceGreaterThanMax
+  | EmptyBlobs
+  | BlobCreateTransaction
+  | TooManyBlobs
+    (max : Usize.t)
+    (have : Usize.t)
+  | BlobVersionNotSupported
+  | EofCrateShouldHaveToAddress
+  | AuthorizationListNotSupported
+  | AuthorizationListInvalidFields
+  | EmptyAuthorizationList
+  | InvalidAuthorizationList
+    (_ : revm_specification.eip7702.links.authorization_list.InvalidAuthorization.t)
+  | Eip2930NotSupported
+  | Eip1559NotSupported
+  | Eip4844NotSupported
+  | Eip7702NotSupported
+  .
+
+  Global Instance IsLink : Link t := {
+    Φ := Ty.path "revm_context_interface::result::InvalidTransaction";
+    φ x :=
+      match x with
+      | PriorityFeeGreaterThanMaxFee  =>
+        Value.StructTuple "revm_context_interface::result::InvalidTransaction::PriorityFeeGreaterThanMaxFee" []
+      | GasPriceLessThanBasefee  =>
+        Value.StructTuple "revm_context_interface::result::InvalidTransaction::GasPriceLessThanBasefee" []
+      | CallerGasLimitMoreThanBlock  =>
+        Value.StructTuple "revm_context_interface::result::InvalidTransaction::CallerGasLimitMoreThanBlock" []
+      | CallGasCostMoreThanGasLimit  =>
+        Value.StructTuple "revm_context_interface::result::InvalidTransaction::CallGasCostMoreThanGasLimit" []
+      | RejectCallerWithCode  =>
+        Value.StructTuple "revm_context_interface::result::InvalidTransaction::RejectCallerWithCode" []
+      | LackOfFundForMaxFee fee balance =>
+        Value.StructRecord "revm_context_interface::result::InvalidTransaction::LackOfFundForMaxFee" [
+          ("fee", φ fee);
+          ("balance", φ balance)
+        ]
+      | OverflowPaymentInTransaction  =>
+        Value.StructTuple "revm_context_interface::result::InvalidTransaction::OverflowPaymentInTransaction" []
+      | NonceOverflowInTransaction  =>
+        Value.StructTuple "revm_context_interface::result::InvalidTransaction::NonceOverflowInTransaction" []
+      | NonceTooHigh tx state =>
+        Value.StructRecord "revm_context_interface::result::InvalidTransaction::NonceTooHigh" [
+          ("tx", φ tx);
+          ("state", φ state)
+        ]
+      | NonceTooLow tx state =>
+        Value.StructRecord "revm_context_interface::result::InvalidTransaction::NonceTooLow" [
+          ("tx", φ tx);
+          ("state", φ state)
+        ]
+      | CreateInitCodeSizeLimit  =>
+        Value.StructTuple "revm_context_interface::result::InvalidTransaction::CreateInitCodeSizeLimit" []
+      | InvalidChainId  =>
+        Value.StructTuple "revm_context_interface::result::InvalidTransaction::InvalidChainId" []
+      | AccessListNotSupported  =>
+        Value.StructTuple "revm_context_interface::result::InvalidTransaction::AccessListNotSupported" []
+      | MaxFeePerBlobGasNotSupported  =>
+        Value.StructTuple "revm_context_interface::result::InvalidTransaction::MaxFeePerBlobGasNotSupported" []
+      | BlobVersionedHashesNotSupported  =>
+        Value.StructTuple "revm_context_interface::result::InvalidTransaction::BlobVersionedHashesNotSupported" []
+      | BlobGasPriceGreaterThanMax  =>
+        Value.StructTuple "revm_context_interface::result::InvalidTransaction::BlobGasPriceGreaterThanMax" []
+      | EmptyBlobs  =>
+        Value.StructTuple "revm_context_interface::result::InvalidTransaction::EmptyBlobs" []
+      | BlobCreateTransaction  =>
+        Value.StructTuple "revm_context_interface::result::InvalidTransaction::BlobCreateTransaction" []
+      | TooManyBlobs max have =>
+        Value.StructRecord "revm_context_interface::result::InvalidTransaction::TooManyBlobs" [
+          ("max", φ max);
+          ("have", φ have)
+        ]
+      | BlobVersionNotSupported  =>
+        Value.StructTuple "revm_context_interface::result::InvalidTransaction::BlobVersionNotSupported" []
+      | EofCrateShouldHaveToAddress  =>
+        Value.StructTuple "revm_context_interface::result::InvalidTransaction::EofCrateShouldHaveToAddress" []
+      | AuthorizationListNotSupported  =>
+        Value.StructTuple "revm_context_interface::result::InvalidTransaction::AuthorizationListNotSupported" []
+      | AuthorizationListInvalidFields  =>
+        Value.StructTuple "revm_context_interface::result::InvalidTransaction::AuthorizationListInvalidFields" []
+      | EmptyAuthorizationList  =>
+        Value.StructTuple "revm_context_interface::result::InvalidTransaction::EmptyAuthorizationList" []
+      | InvalidAuthorizationList γ0 =>
+        Value.StructTuple "revm_context_interface::result::InvalidTransaction::InvalidAuthorizationList" [
+          φ γ0
+        ]
+      | Eip2930NotSupported  =>
+        Value.StructTuple "revm_context_interface::result::InvalidTransaction::Eip2930NotSupported" []
+      | Eip1559NotSupported  =>
+        Value.StructTuple "revm_context_interface::result::InvalidTransaction::Eip1559NotSupported" []
+      | Eip4844NotSupported  =>
+        Value.StructTuple "revm_context_interface::result::InvalidTransaction::Eip4844NotSupported" []
+      | Eip7702NotSupported  =>
+        Value.StructTuple "revm_context_interface::result::InvalidTransaction::Eip7702NotSupported" []
+      end
+  }.
+End InvalidTransaction.
+
+Module InvalidHeader.
+  Inductive t : Set :=
+  | PrevrandaoNotSet
+  | ExcessBlobGasNotSet
+  .
+
+  Global Instance IsLink : Link t := {
+    Φ := Ty.path "revm_context_interface::result::InvalidHeader";
+    φ x :=
+      match x with
+      | PrevrandaoNotSet  =>
+        Value.StructTuple "revm_context_interface::result::InvalidHeader::PrevrandaoNotSet" []
+      | ExcessBlobGasNotSet  =>
+        Value.StructTuple "revm_context_interface::result::InvalidHeader::ExcessBlobGasNotSet" []
+      end
+  }.
+End InvalidHeader.
+
+Module SuccessReason.
+  Inductive t : Set :=
+  | Stop
+  | Return
+  | SelfDestruct
+  | EofReturnContract
+  .
+
+  Global Instance IsLink : Link t := {
+    Φ := Ty.path "revm_context_interface::result::SuccessReason";
+    φ x :=
+      match x with
+      | Stop  =>
+        Value.StructTuple "revm_context_interface::result::SuccessReason::Stop" []
+      | Return  =>
+        Value.StructTuple "revm_context_interface::result::SuccessReason::Return" []
+      | SelfDestruct  =>
+        Value.StructTuple "revm_context_interface::result::SuccessReason::SelfDestruct" []
+      | EofReturnContract  =>
+        Value.StructTuple "revm_context_interface::result::SuccessReason::EofReturnContract" []
+      end
+  }.
+End SuccessReason.
+
+Module HaltReason.
+  Inductive t : Set :=
+  | OutOfGas
+    (_ : revm_context_interface.links.result.OutOfGasError.t)
+  | OpcodeNotFound
+  | InvalidFEOpcode
+  | InvalidJump
+  | NotActivated
+  | StackUnderflow
+  | StackOverflow
+  | OutOfOffset
+  | CreateCollision
+  | PrecompileError
+  | NonceOverflow
+  | CreateContractSizeLimit
+  | CreateContractStartingWithEF
+  | CreateInitCodeSizeLimit
+  | OverflowPayment
+  | StateChangeDuringStaticCall
+  | CallNotAllowedInsideStatic
+  | OutOfFunds
+  | CallTooDeep
+  | EofAuxDataOverflow
+  | EofAuxDataTooSmall
+  | SubRoutineStackOverflow
+  | InvalidEXTCALLTarget
+  .
+
+  Global Instance IsLink : Link t := {
+    Φ := Ty.path "revm_context_interface::result::HaltReason";
+    φ x :=
+      match x with
+      | OutOfGas γ0 =>
+        Value.StructTuple "revm_context_interface::result::HaltReason::OutOfGas" [
+          φ γ0
+        ]
+      | OpcodeNotFound  =>
+        Value.StructTuple "revm_context_interface::result::HaltReason::OpcodeNotFound" []
+      | InvalidFEOpcode  =>
+        Value.StructTuple "revm_context_interface::result::HaltReason::InvalidFEOpcode" []
+      | InvalidJump  =>
+        Value.StructTuple "revm_context_interface::result::HaltReason::InvalidJump" []
+      | NotActivated  =>
+        Value.StructTuple "revm_context_interface::result::HaltReason::NotActivated" []
+      | StackUnderflow  =>
+        Value.StructTuple "revm_context_interface::result::HaltReason::StackUnderflow" []
+      | StackOverflow  =>
+        Value.StructTuple "revm_context_interface::result::HaltReason::StackOverflow" []
+      | OutOfOffset  =>
+        Value.StructTuple "revm_context_interface::result::HaltReason::OutOfOffset" []
+      | CreateCollision  =>
+        Value.StructTuple "revm_context_interface::result::HaltReason::CreateCollision" []
+      | PrecompileError  =>
+        Value.StructTuple "revm_context_interface::result::HaltReason::PrecompileError" []
+      | NonceOverflow  =>
+        Value.StructTuple "revm_context_interface::result::HaltReason::NonceOverflow" []
+      | CreateContractSizeLimit  =>
+        Value.StructTuple "revm_context_interface::result::HaltReason::CreateContractSizeLimit" []
+      | CreateContractStartingWithEF  =>
+        Value.StructTuple "revm_context_interface::result::HaltReason::CreateContractStartingWithEF" []
+      | CreateInitCodeSizeLimit  =>
+        Value.StructTuple "revm_context_interface::result::HaltReason::CreateInitCodeSizeLimit" []
+      | OverflowPayment  =>
+        Value.StructTuple "revm_context_interface::result::HaltReason::OverflowPayment" []
+      | StateChangeDuringStaticCall  =>
+        Value.StructTuple "revm_context_interface::result::HaltReason::StateChangeDuringStaticCall" []
+      | CallNotAllowedInsideStatic  =>
+        Value.StructTuple "revm_context_interface::result::HaltReason::CallNotAllowedInsideStatic" []
+      | OutOfFunds  =>
+        Value.StructTuple "revm_context_interface::result::HaltReason::OutOfFunds" []
+      | CallTooDeep  =>
+        Value.StructTuple "revm_context_interface::result::HaltReason::CallTooDeep" []
+      | EofAuxDataOverflow  =>
+        Value.StructTuple "revm_context_interface::result::HaltReason::EofAuxDataOverflow" []
+      | EofAuxDataTooSmall  =>
+        Value.StructTuple "revm_context_interface::result::HaltReason::EofAuxDataTooSmall" []
+      | SubRoutineStackOverflow  =>
+        Value.StructTuple "revm_context_interface::result::HaltReason::SubRoutineStackOverflow" []
+      | InvalidEXTCALLTarget  =>
+        Value.StructTuple "revm_context_interface::result::HaltReason::InvalidEXTCALLTarget" []
+      end
+  }.
+End HaltReason.
+
+Module OutOfGasError.
+  Inductive t : Set :=
+  | Basic
+  | MemoryLimit
+  | Memory
+  | Precompile
+  | InvalidOperand
+  | ReentrancySentry
+  .
+
+  Global Instance IsLink : Link t := {
+    Φ := Ty.path "revm_context_interface::result::OutOfGasError";
+    φ x :=
+      match x with
+      | Basic  =>
+        Value.StructTuple "revm_context_interface::result::OutOfGasError::Basic" []
+      | MemoryLimit  =>
+        Value.StructTuple "revm_context_interface::result::OutOfGasError::MemoryLimit" []
+      | Memory  =>
+        Value.StructTuple "revm_context_interface::result::OutOfGasError::Memory" []
+      | Precompile  =>
+        Value.StructTuple "revm_context_interface::result::OutOfGasError::Precompile" []
+      | InvalidOperand  =>
+        Value.StructTuple "revm_context_interface::result::OutOfGasError::InvalidOperand" []
+      | ReentrancySentry  =>
+        Value.StructTuple "revm_context_interface::result::OutOfGasError::ReentrancySentry" []
+      end
+  }.
+End OutOfGasError.
+
+Module TransferError.
+  Inductive t : Set :=
+  | OutOfFunds
+  | OverflowPayment
+  | CreateCollision
+  .
+
+  Global Instance IsLink : Link t := {
+    Φ := Ty.path "revm_context_interface::journaled_state::TransferError";
+    φ x :=
+      match x with
+      | OutOfFunds  =>
+        Value.StructTuple "revm_context_interface::journaled_state::TransferError::OutOfFunds" []
+      | OverflowPayment  =>
+        Value.StructTuple "revm_context_interface::journaled_state::TransferError::OverflowPayment" []
+      | CreateCollision  =>
+        Value.StructTuple "revm_context_interface::journaled_state::TransferError::CreateCollision" []
+      end
+  }.
+End TransferError.
+
+Module JournalCheckpoint.
+  Record t : Set := {
+    log_i: Usize.t;
+    journal_i: Usize.t;
+  }.
+
+  Global Instance IsLink : Link t := {
+    Φ := Ty.path "revm_context_interface::journaled_state::JournalCheckpoint";
+    φ '(Build_t log_i journal_i) :=
+      Value.StructRecord "revm_context_interface::journaled_state::JournalCheckpoint" [
+        ("log_i", φ log_i);
+        ("journal_i", φ journal_i)
+      ]
+  }.
+End JournalCheckpoint.
+
+Module StateLoad.
+  Record t {T: Set} : Set := {
+    data: T;
+    is_cold: bool;
+  }.
+  Arguments Build_t {_}.
+  Arguments t : clear implicits.
+
+  Global Instance IsLink {T: Set} `{Link T} : Link (t T) := {
+    Φ := Ty.path "revm_context_interface::journaled_state::StateLoad";
+    φ '(Build_t data is_cold) :=
+      Value.StructRecord "revm_context_interface::journaled_state::StateLoad" [
+        ("data", φ data);
+        ("is_cold", φ is_cold)
+      ]
+  }.
+End StateLoad.
+
+Module AccountLoad.
+  Record t : Set := {
+    load: revm_context_interface.links.journaled_state.Eip7702CodeLoad.t ();
+    is_empty: bool;
+  }.
+
+  Global Instance IsLink : Link t := {
+    Φ := Ty.path "revm_context_interface::journaled_state::AccountLoad";
+    φ '(Build_t load is_empty) :=
+      Value.StructRecord "revm_context_interface::journaled_state::AccountLoad" [
+        ("load", φ load);
+        ("is_empty", φ is_empty)
+      ]
+  }.
+End AccountLoad.
+
+Module Eip7702CodeLoad.
+  Record t {T: Set} : Set := {
+    state_load: revm_context_interface.links.journaled_state.StateLoad.t T;
+    is_delegate_account_cold: core.links.option.Option.t bool;
+  }.
+  Arguments Build_t {_}.
+  Arguments t : clear implicits.
+
+  Global Instance IsLink {T: Set} `{Link T} : Link (t T) := {
+    Φ := Ty.path "revm_context_interface::journaled_state::Eip7702CodeLoad";
+    φ '(Build_t state_load is_delegate_account_cold) :=
+      Value.StructRecord "revm_context_interface::journaled_state::Eip7702CodeLoad" [
+        ("state_load", φ state_load);
+        ("is_delegate_account_cold", φ is_delegate_account_cold)
+      ]
+  }.
+End Eip7702CodeLoad.
+
+Module SStoreResult.
+  Record t : Set := {
+    original_value: ruint.Uint.t 256 4;
+    present_value: ruint.Uint.t 256 4;
+    new_value: ruint.Uint.t 256 4;
+  }.
+
+  Global Instance IsLink : Link t := {
+    Φ := Ty.path "revm_context_interface::host::SStoreResult";
+    φ '(Build_t original_value present_value new_value) :=
+      Value.StructRecord "revm_context_interface::host::SStoreResult" [
+        ("original_value", φ original_value);
+        ("present_value", φ present_value);
+        ("new_value", φ new_value)
+      ]
+  }.
+End SStoreResult.
+
+Module SelfDestructResult.
+  Record t : Set := {
+    had_value: bool;
+    target_exists: bool;
+    previously_destroyed: bool;
+  }.
+
+  Global Instance IsLink : Link t := {
+    Φ := Ty.path "revm_context_interface::host::SelfDestructResult";
+    φ '(Build_t had_value target_exists previously_destroyed) :=
+      Value.StructRecord "revm_context_interface::host::SelfDestructResult" [
+        ("had_value", φ had_value);
+        ("target_exists", φ target_exists);
+        ("previously_destroyed", φ previously_destroyed)
+      ]
+  }.
+End SelfDestructResult.
+
+Module TransactionType.
+  Inductive t : Set :=
+  | Legacy
+  | Eip2930
+  | Eip1559
+  | Eip4844
+  | Eip7702
+  | Custom
+  .
+
+  Global Instance IsLink : Link t := {
+    Φ := Ty.path "revm_context_interface::transaction::transaction_type::TransactionType";
+    φ x :=
+      match x with
+      | Legacy  =>
+        Value.StructTuple "revm_context_interface::transaction::transaction_type::TransactionType::Legacy" []
+      | Eip2930  =>
+        Value.StructTuple "revm_context_interface::transaction::transaction_type::TransactionType::Eip2930" []
+      | Eip1559  =>
+        Value.StructTuple "revm_context_interface::transaction::transaction_type::TransactionType::Eip1559" []
+      | Eip4844  =>
+        Value.StructTuple "revm_context_interface::transaction::transaction_type::TransactionType::Eip4844" []
+      | Eip7702  =>
+        Value.StructTuple "revm_context_interface::transaction::transaction_type::TransactionType::Eip7702" []
+      | Custom  =>
+        Value.StructTuple "revm_context_interface::transaction::transaction_type::TransactionType::Custom" []
+      end
+  }.
+End TransactionType.
+
+Module DummyHost.
+  Record t {BLOCK TX CFG: Set} : Set := {
+    tx: TX;
+    block: BLOCK;
+    cfg: CFG;
+    storage: hashbrown.links.map.HashMap.t (ruint.Uint.t 256 4) (ruint.Uint.t 256 4) foldhash.seed.links.fast.RandomState.t hashbrown.raw.alloc.links.inner.Global.t;
+    transient_storage: hashbrown.links.map.HashMap.t (ruint.Uint.t 256 4) (ruint.Uint.t 256 4) foldhash.seed.links.fast.RandomState.t hashbrown.raw.alloc.links.inner.Global.t;
+    log: alloc.links.vec.Vec.t (alloy_primitives.links.log.Log.t alloy_primitives.links.log.LogData.t) alloc.links.alloc.Global.t;
+  }.
+  Arguments Build_t {_ _ _}.
+  Arguments t : clear implicits.
+
+  Global Instance IsLink {BLOCK TX CFG: Set} `{Link BLOCK} `{Link TX} `{Link CFG} : Link (t BLOCK TX CFG) := {
+    Φ := Ty.path "revm_context_interface::host::dummy::DummyHost";
+    φ '(Build_t tx block cfg storage transient_storage log) :=
+      Value.StructRecord "revm_context_interface::host::dummy::DummyHost" [
+        ("tx", φ tx);
+        ("block", φ block);
+        ("cfg", φ cfg);
+        ("storage", φ storage);
+        ("transient_storage", φ transient_storage);
+        ("log", φ log)
+      ]
+  }.
+End DummyHost.
+
+Module BlobExcessGasAndPrice.
+  Record t : Set := {
+    excess_blob_gas: U64.t;
+    blob_gasprice: U128.t;
+  }.
+
+  Global Instance IsLink : Link t := {
+    Φ := Ty.path "revm_context_interface::block::blob::BlobExcessGasAndPrice";
+    φ '(Build_t excess_blob_gas blob_gasprice) :=
+      Value.StructRecord "revm_context_interface::block::blob::BlobExcessGasAndPrice" [
+        ("excess_blob_gas", φ excess_blob_gas);
+        ("blob_gasprice", φ blob_gasprice)
+      ]
+  }.
+End BlobExcessGasAndPrice.
+
+Module SpecId.
+  Inductive t : Set :=
+  | FRONTIER
+  | FRONTIER_THAWING
+  | HOMESTEAD
+  | DAO_FORK
+  | TANGERINE
+  | SPURIOUS_DRAGON
+  | BYZANTIUM
+  | CONSTANTINOPLE
+  | PETERSBURG
+  | ISTANBUL
+  | MUIR_GLACIER
+  | BERLIN
+  | LONDON
+  | ARROW_GLACIER
+  | GRAY_GLACIER
+  | MERGE
+  | SHANGHAI
+  | CANCUN
+  | PRAGUE
+  | OSAKA
+  | LATEST
+  .
+
+  Global Instance IsLink : Link t := {
+    Φ := Ty.path "revm_specification::hardfork::SpecId";
+    φ x :=
+      match x with
+      | FRONTIER  =>
+        Value.StructTuple "revm_specification::hardfork::SpecId::FRONTIER" []
+      | FRONTIER_THAWING  =>
+        Value.StructTuple "revm_specification::hardfork::SpecId::FRONTIER_THAWING" []
+      | HOMESTEAD  =>
+        Value.StructTuple "revm_specification::hardfork::SpecId::HOMESTEAD" []
+      | DAO_FORK  =>
+        Value.StructTuple "revm_specification::hardfork::SpecId::DAO_FORK" []
+      | TANGERINE  =>
+        Value.StructTuple "revm_specification::hardfork::SpecId::TANGERINE" []
+      | SPURIOUS_DRAGON  =>
+        Value.StructTuple "revm_specification::hardfork::SpecId::SPURIOUS_DRAGON" []
+      | BYZANTIUM  =>
+        Value.StructTuple "revm_specification::hardfork::SpecId::BYZANTIUM" []
+      | CONSTANTINOPLE  =>
+        Value.StructTuple "revm_specification::hardfork::SpecId::CONSTANTINOPLE" []
+      | PETERSBURG  =>
+        Value.StructTuple "revm_specification::hardfork::SpecId::PETERSBURG" []
+      | ISTANBUL  =>
+        Value.StructTuple "revm_specification::hardfork::SpecId::ISTANBUL" []
+      | MUIR_GLACIER  =>
+        Value.StructTuple "revm_specification::hardfork::SpecId::MUIR_GLACIER" []
+      | BERLIN  =>
+        Value.StructTuple "revm_specification::hardfork::SpecId::BERLIN" []
+      | LONDON  =>
+        Value.StructTuple "revm_specification::hardfork::SpecId::LONDON" []
+      | ARROW_GLACIER  =>
+        Value.StructTuple "revm_specification::hardfork::SpecId::ARROW_GLACIER" []
+      | GRAY_GLACIER  =>
+        Value.StructTuple "revm_specification::hardfork::SpecId::GRAY_GLACIER" []
+      | MERGE  =>
+        Value.StructTuple "revm_specification::hardfork::SpecId::MERGE" []
+      | SHANGHAI  =>
+        Value.StructTuple "revm_specification::hardfork::SpecId::SHANGHAI" []
+      | CANCUN  =>
+        Value.StructTuple "revm_specification::hardfork::SpecId::CANCUN" []
+      | PRAGUE  =>
+        Value.StructTuple "revm_specification::hardfork::SpecId::PRAGUE" []
+      | OSAKA  =>
+        Value.StructTuple "revm_specification::hardfork::SpecId::OSAKA" []
+      | LATEST  =>
+        Value.StructTuple "revm_specification::hardfork::SpecId::LATEST" []
+      end
+  }.
+End SpecId.
+
+Module AuthorizationList.
+  Inductive t : Set :=
+  | Signed
+    (_ : alloc.links.vec.Vec.t alloy_eip7702.links.auth_list.SignedAuthorization.t alloc.links.alloc.Global.t)
+  | Recovered
+    (_ : alloc.links.vec.Vec.t revm_specification.eip7702.links.recovered_authorization.RecoveredAuthorization.t alloc.links.alloc.Global.t)
+  .
+
+  Global Instance IsLink : Link t := {
+    Φ := Ty.path "revm_specification::eip7702::authorization_list::AuthorizationList";
+    φ x :=
+      match x with
+      | Signed γ0 =>
+        Value.StructTuple "revm_specification::eip7702::authorization_list::AuthorizationList::Signed" [
+          φ γ0
+        ]
+      | Recovered γ0 =>
+        Value.StructTuple "revm_specification::eip7702::authorization_list::AuthorizationList::Recovered" [
+          φ γ0
+        ]
+      end
+  }.
+End AuthorizationList.
+
+Module InvalidAuthorization.
+  Inductive t : Set :=
+  | InvalidChainId
+  | InvalidYParity
+  | Eip2InvalidSValue
+  .
+
+  Global Instance IsLink : Link t := {
+    Φ := Ty.path "revm_specification::eip7702::authorization_list::InvalidAuthorization";
+    φ x :=
+      match x with
+      | InvalidChainId  =>
+        Value.StructTuple "revm_specification::eip7702::authorization_list::InvalidAuthorization::InvalidChainId" []
+      | InvalidYParity  =>
+        Value.StructTuple "revm_specification::eip7702::authorization_list::InvalidAuthorization::InvalidYParity" []
+      | Eip2InvalidSValue  =>
+        Value.StructTuple "revm_specification::eip7702::authorization_list::InvalidAuthorization::Eip2InvalidSValue" []
+      end
+  }.
+End InvalidAuthorization.
+
+Module RecoveredAuthorization.
+  Record t : Set := {
+    inner: alloy_eip7702.links.auth_list.SignedAuthorization.t;
+    authority: core.links.option.Option.t alloy_primitives.bits.links.address.Address.t;
+  }.
+
+  Global Instance IsLink : Link t := {
+    Φ := Ty.path "revm_specification::eip7702::recovered_authorization::RecoveredAuthorization";
+    φ '(Build_t inner authority) :=
+      Value.StructRecord "revm_specification::eip7702::recovered_authorization::RecoveredAuthorization" [
+        ("inner", φ inner);
+        ("authority", φ authority)
+      ]
+  }.
+End RecoveredAuthorization.
+
+Module PrecompileOutput.
+  Record t : Set := {
+    gas_used: U64.t;
+    bytes: alloy_primitives.links.bytes_.Bytes.t;
+  }.
+
+  Global Instance IsLink : Link t := {
+    Φ := Ty.path "revm_precompile::interface::PrecompileOutput";
+    φ '(Build_t gas_used bytes) :=
+      Value.StructRecord "revm_precompile::interface::PrecompileOutput" [
+        ("gas_used", φ gas_used);
+        ("bytes", φ bytes)
+      ]
+  }.
+End PrecompileOutput.
+
+Module PrecompileErrors.
+  Inductive t : Set :=
+  | Error
+    (_ : revm_precompile.links.interface.PrecompileError.t)
+  | Fatal
+    (msg : alloc.links.string.String.t)
+  .
+
+  Global Instance IsLink : Link t := {
+    Φ := Ty.path "revm_precompile::interface::PrecompileErrors";
+    φ x :=
+      match x with
+      | Error γ0 =>
+        Value.StructTuple "revm_precompile::interface::PrecompileErrors::Error" [
+          φ γ0
+        ]
+      | Fatal msg =>
+        Value.StructRecord "revm_precompile::interface::PrecompileErrors::Fatal" [
+          ("msg", φ msg)
+        ]
+      end
+  }.
+End PrecompileErrors.
+
+Module PrecompileError.
+  Inductive t : Set :=
+  | OutOfGas
+  | Blake2WrongLength
+  | Blake2WrongFinalIndicatorFlag
+  | ModexpExpOverflow
+  | ModexpBaseOverflow
+  | ModexpModOverflow
+  | Bn128FieldPointNotAMember
+  | Bn128AffineGFailedToCreate
+  | Bn128PairLength
+  | BlobInvalidInputLength
+  | BlobMismatchedVersion
+  | BlobVerifyKzgProofFailed
+  | Other
+    (_ : alloc.links.string.String.t)
+  .
+
+  Global Instance IsLink : Link t := {
+    Φ := Ty.path "revm_precompile::interface::PrecompileError";
+    φ x :=
+      match x with
+      | OutOfGas  =>
+        Value.StructTuple "revm_precompile::interface::PrecompileError::OutOfGas" []
+      | Blake2WrongLength  =>
+        Value.StructTuple "revm_precompile::interface::PrecompileError::Blake2WrongLength" []
+      | Blake2WrongFinalIndicatorFlag  =>
+        Value.StructTuple "revm_precompile::interface::PrecompileError::Blake2WrongFinalIndicatorFlag" []
+      | ModexpExpOverflow  =>
+        Value.StructTuple "revm_precompile::interface::PrecompileError::ModexpExpOverflow" []
+      | ModexpBaseOverflow  =>
+        Value.StructTuple "revm_precompile::interface::PrecompileError::ModexpBaseOverflow" []
+      | ModexpModOverflow  =>
+        Value.StructTuple "revm_precompile::interface::PrecompileError::ModexpModOverflow" []
+      | Bn128FieldPointNotAMember  =>
+        Value.StructTuple "revm_precompile::interface::PrecompileError::Bn128FieldPointNotAMember" []
+      | Bn128AffineGFailedToCreate  =>
+        Value.StructTuple "revm_precompile::interface::PrecompileError::Bn128AffineGFailedToCreate" []
+      | Bn128PairLength  =>
+        Value.StructTuple "revm_precompile::interface::PrecompileError::Bn128PairLength" []
+      | BlobInvalidInputLength  =>
+        Value.StructTuple "revm_precompile::interface::PrecompileError::BlobInvalidInputLength" []
+      | BlobMismatchedVersion  =>
+        Value.StructTuple "revm_precompile::interface::PrecompileError::BlobMismatchedVersion" []
+      | BlobVerifyKzgProofFailed  =>
+        Value.StructTuple "revm_precompile::interface::PrecompileError::BlobVerifyKzgProofFailed" []
+      | Other γ0 =>
+        Value.StructTuple "revm_precompile::interface::PrecompileError::Other" [
+          φ γ0
+        ]
+      end
+  }.
+End PrecompileError.
+
+Module Precompiles.
+  Record t : Set := {
+    inner: std.collections.hash.links.map.HashMap.t alloy_primitives.bits.links.address.Address.t (Function2.t (Ref.t Pointer.Kind.Ref alloy_primitives.links.bytes_.Bytes.t) U64.t (core.links.result.Result.t revm_precompile.links.interface.PrecompileOutput.t revm_precompile.links.interface.PrecompileErrors.t)) std.hash.links.random.RandomState.t;
+    addresses: std.collections.hash.links.set.HashSet.t alloy_primitives.bits.links.address.Address.t std.hash.links.random.RandomState.t;
+  }.
+
+  Global Instance IsLink : Link t := {
+    Φ := Ty.path "revm_precompile::Precompiles";
+    φ '(Build_t inner addresses) :=
+      Value.StructRecord "revm_precompile::Precompiles" [
+        ("inner", φ inner);
+        ("addresses", φ addresses)
+      ]
+  }.
+End Precompiles.
+
+Module PrecompileSpecId.
+  Inductive t : Set :=
+  | HOMESTEAD
+  | BYZANTIUM
+  | ISTANBUL
+  | BERLIN
+  | CANCUN
+  | PRAGUE
+  | LATEST
+  .
+
+  Global Instance IsLink : Link t := {
+    Φ := Ty.path "revm_precompile::PrecompileSpecId";
+    φ x :=
+      match x with
+      | HOMESTEAD  =>
+        Value.StructTuple "revm_precompile::PrecompileSpecId::HOMESTEAD" []
+      | BYZANTIUM  =>
+        Value.StructTuple "revm_precompile::PrecompileSpecId::BYZANTIUM" []
+      | ISTANBUL  =>
+        Value.StructTuple "revm_precompile::PrecompileSpecId::ISTANBUL" []
+      | BERLIN  =>
+        Value.StructTuple "revm_precompile::PrecompileSpecId::BERLIN" []
+      | CANCUN  =>
+        Value.StructTuple "revm_precompile::PrecompileSpecId::CANCUN" []
+      | PRAGUE  =>
+        Value.StructTuple "revm_precompile::PrecompileSpecId::PRAGUE" []
+      | LATEST  =>
+        Value.StructTuple "revm_precompile::PrecompileSpecId::LATEST" []
+      end
+  }.
+End PrecompileSpecId.
+
+Module Eip7702Bytecode.
+  Record t : Set := {
+    delegated_address: alloy_primitives.bits.links.address.Address.t;
+    version: U8.t;
+    raw: alloy_primitives.links.bytes_.Bytes.t;
+  }.
+
+  Global Instance IsLink : Link t := {
+    Φ := Ty.path "revm_bytecode::eip7702::Eip7702Bytecode";
+    φ '(Build_t delegated_address version raw) :=
+      Value.StructRecord "revm_bytecode::eip7702::Eip7702Bytecode" [
+        ("delegated_address", φ delegated_address);
+        ("version", φ version);
+        ("raw", φ raw)
+      ]
+  }.
+End Eip7702Bytecode.
+
+Module Eip7702DecodeError.
+  Inductive t : Set :=
+  | InvalidLength
+  | InvalidMagic
+  | UnsupportedVersion
+  .
+
+  Global Instance IsLink : Link t := {
+    Φ := Ty.path "revm_bytecode::eip7702::Eip7702DecodeError";
+    φ x :=
+      match x with
+      | InvalidLength  =>
+        Value.StructTuple "revm_bytecode::eip7702::Eip7702DecodeError::InvalidLength" []
+      | InvalidMagic  =>
+        Value.StructTuple "revm_bytecode::eip7702::Eip7702DecodeError::InvalidMagic" []
+      | UnsupportedVersion  =>
+        Value.StructTuple "revm_bytecode::eip7702::Eip7702DecodeError::UnsupportedVersion" []
+      end
+  }.
+End Eip7702DecodeError.
+
+Module Bytecode.
+  Inductive t : Set :=
+  | LegacyAnalyzed
+    (_ : revm_bytecode.legacy.links.analyzed.LegacyAnalyzedBytecode.t)
+  | Eof
+    (_ : alloc.links.sync.Arc.t revm_bytecode.links.eof.Eof.t alloc.links.alloc.Global.t)
+  | Eip7702
+    (_ : revm_bytecode.links.eip7702.Eip7702Bytecode.t)
+  .
+
+  Global Instance IsLink : Link t := {
+    Φ := Ty.path "revm_bytecode::bytecode::Bytecode";
+    φ x :=
+      match x with
+      | LegacyAnalyzed γ0 =>
+        Value.StructTuple "revm_bytecode::bytecode::Bytecode::LegacyAnalyzed" [
+          φ γ0
+        ]
+      | Eof γ0 =>
+        Value.StructTuple "revm_bytecode::bytecode::Bytecode::Eof" [
+          φ γ0
+        ]
+      | Eip7702 γ0 =>
+        Value.StructTuple "revm_bytecode::bytecode::Bytecode::Eip7702" [
+          φ γ0
+        ]
+      end
+  }.
+End Bytecode.
+
+Module Eof.
+  Record t : Set := {
+    header: revm_bytecode.eof.links.header.EofHeader.t;
+    body: revm_bytecode.eof.links.body.EofBody.t;
+    raw: alloy_primitives.links.bytes_.Bytes.t;
+  }.
+
+  Global Instance IsLink : Link t := {
+    Φ := Ty.path "revm_bytecode::eof::Eof";
+    φ '(Build_t header body raw) :=
+      Value.StructRecord "revm_bytecode::eof::Eof" [
+        ("header", φ header);
+        ("body", φ body);
+        ("raw", φ raw)
+      ]
+  }.
+End Eof.
+
+Module EofDecodeError.
+  Inductive t : Set :=
+  | MissingInput
+  | MissingBodyWithoutData
+  | DanglingData
+  | InvalidTypesSection
+  | InvalidTypesSectionSize
+  | InvalidEOFMagicNumber
+  | InvalidEOFVersion
+  | InvalidTypesKind
+  | InvalidCodeKind
+  | InvalidTerminalByte
+  | InvalidDataKind
+  | InvalidKindAfterCode
+  | MismatchCodeAndTypesSize
+  | NonSizes
+  | ShortInputForSizes
+  | ZeroSize
+  | TooManyCodeSections
+  | ZeroCodeSections
+  | TooManyContainerSections
+  | InvalidEOFSize
+  .
+
+  Global Instance IsLink : Link t := {
+    Φ := Ty.path "revm_bytecode::eof::EofDecodeError";
+    φ x :=
+      match x with
+      | MissingInput  =>
+        Value.StructTuple "revm_bytecode::eof::EofDecodeError::MissingInput" []
+      | MissingBodyWithoutData  =>
+        Value.StructTuple "revm_bytecode::eof::EofDecodeError::MissingBodyWithoutData" []
+      | DanglingData  =>
+        Value.StructTuple "revm_bytecode::eof::EofDecodeError::DanglingData" []
+      | InvalidTypesSection  =>
+        Value.StructTuple "revm_bytecode::eof::EofDecodeError::InvalidTypesSection" []
+      | InvalidTypesSectionSize  =>
+        Value.StructTuple "revm_bytecode::eof::EofDecodeError::InvalidTypesSectionSize" []
+      | InvalidEOFMagicNumber  =>
+        Value.StructTuple "revm_bytecode::eof::EofDecodeError::InvalidEOFMagicNumber" []
+      | InvalidEOFVersion  =>
+        Value.StructTuple "revm_bytecode::eof::EofDecodeError::InvalidEOFVersion" []
+      | InvalidTypesKind  =>
+        Value.StructTuple "revm_bytecode::eof::EofDecodeError::InvalidTypesKind" []
+      | InvalidCodeKind  =>
+        Value.StructTuple "revm_bytecode::eof::EofDecodeError::InvalidCodeKind" []
+      | InvalidTerminalByte  =>
+        Value.StructTuple "revm_bytecode::eof::EofDecodeError::InvalidTerminalByte" []
+      | InvalidDataKind  =>
+        Value.StructTuple "revm_bytecode::eof::EofDecodeError::InvalidDataKind" []
+      | InvalidKindAfterCode  =>
+        Value.StructTuple "revm_bytecode::eof::EofDecodeError::InvalidKindAfterCode" []
+      | MismatchCodeAndTypesSize  =>
+        Value.StructTuple "revm_bytecode::eof::EofDecodeError::MismatchCodeAndTypesSize" []
+      | NonSizes  =>
+        Value.StructTuple "revm_bytecode::eof::EofDecodeError::NonSizes" []
+      | ShortInputForSizes  =>
+        Value.StructTuple "revm_bytecode::eof::EofDecodeError::ShortInputForSizes" []
+      | ZeroSize  =>
+        Value.StructTuple "revm_bytecode::eof::EofDecodeError::ZeroSize" []
+      | TooManyCodeSections  =>
+        Value.StructTuple "revm_bytecode::eof::EofDecodeError::TooManyCodeSections" []
+      | ZeroCodeSections  =>
+        Value.StructTuple "revm_bytecode::eof::EofDecodeError::ZeroCodeSections" []
+      | TooManyContainerSections  =>
+        Value.StructTuple "revm_bytecode::eof::EofDecodeError::TooManyContainerSections" []
+      | InvalidEOFSize  =>
+        Value.StructTuple "revm_bytecode::eof::EofDecodeError::InvalidEOFSize" []
+      end
+  }.
+End EofDecodeError.
+
+Module BytecodeDecodeError.
+  Inductive t : Set :=
+  | Eof
+    (_ : revm_bytecode.links.eof.EofDecodeError.t)
+  | Eip7702
+    (_ : revm_bytecode.links.eip7702.Eip7702DecodeError.t)
+  .
+
+  Global Instance IsLink : Link t := {
+    Φ := Ty.path "revm_bytecode::decode_errors::BytecodeDecodeError";
+    φ x :=
+      match x with
+      | Eof γ0 =>
+        Value.StructTuple "revm_bytecode::decode_errors::BytecodeDecodeError::Eof" [
+          φ γ0
+        ]
+      | Eip7702 γ0 =>
+        Value.StructTuple "revm_bytecode::decode_errors::BytecodeDecodeError::Eip7702" [
+          φ γ0
+        ]
+      end
+  }.
+End BytecodeDecodeError.
+
+Module LegacyAnalyzedBytecode.
+  Record t : Set := {
+    bytecode: alloy_primitives.links.bytes_.Bytes.t;
+    original_len: Usize.t;
+    jump_table: revm_bytecode.legacy.links.jump_map.JumpTable.t;
+  }.
+
+  Global Instance IsLink : Link t := {
+    Φ := Ty.path "revm_bytecode::legacy::analyzed::LegacyAnalyzedBytecode";
+    φ '(Build_t bytecode original_len jump_table) :=
+      Value.StructRecord "revm_bytecode::legacy::analyzed::LegacyAnalyzedBytecode" [
+        ("bytecode", φ bytecode);
+        ("original_len", φ original_len);
+        ("jump_table", φ jump_table)
+      ]
+  }.
+End LegacyAnalyzedBytecode.
+
+Module EofHeader.
+  Record t : Set := {
+    types_size: U16.t;
+    code_sizes: alloc.links.vec.Vec.t U16.t alloc.links.alloc.Global.t;
+    container_sizes: alloc.links.vec.Vec.t U16.t alloc.links.alloc.Global.t;
+    data_size: U16.t;
+    sum_code_sizes: Usize.t;
+    sum_container_sizes: Usize.t;
+  }.
+
+  Global Instance IsLink : Link t := {
+    Φ := Ty.path "revm_bytecode::eof::header::EofHeader";
+    φ '(Build_t types_size code_sizes container_sizes data_size sum_code_sizes sum_container_sizes) :=
+      Value.StructRecord "revm_bytecode::eof::header::EofHeader" [
+        ("types_size", φ types_size);
+        ("code_sizes", φ code_sizes);
+        ("container_sizes", φ container_sizes);
+        ("data_size", φ data_size);
+        ("sum_code_sizes", φ sum_code_sizes);
+        ("sum_container_sizes", φ sum_container_sizes)
+      ]
+  }.
+End EofHeader.
+
+Module EofBody.
+  Record t : Set := {
+    types_section: alloc.links.vec.Vec.t revm_bytecode.eof.links.types_section.TypesSection.t alloc.links.alloc.Global.t;
+    code_section: alloc.links.vec.Vec.t Usize.t alloc.links.alloc.Global.t;
+    code: alloy_primitives.links.bytes_.Bytes.t;
+    container_section: alloc.links.vec.Vec.t alloy_primitives.links.bytes_.Bytes.t alloc.links.alloc.Global.t;
+    data_section: alloy_primitives.links.bytes_.Bytes.t;
+    is_data_filled: bool;
+  }.
+
+  Global Instance IsLink : Link t := {
+    Φ := Ty.path "revm_bytecode::eof::body::EofBody";
+    φ '(Build_t types_section code_section code container_section data_section is_data_filled) :=
+      Value.StructRecord "revm_bytecode::eof::body::EofBody" [
+        ("types_section", φ types_section);
+        ("code_section", φ code_section);
+        ("code", φ code);
+        ("container_section", φ container_section);
+        ("data_section", φ data_section);
+        ("is_data_filled", φ is_data_filled)
+      ]
+  }.
+End EofBody.
+
+Module EofError.
+  Inductive t : Set :=
+  | Decode
+    (_ : revm_bytecode.links.eof.EofDecodeError.t)
+  | Validation
+    (_ : revm_bytecode.eof.links.verification.EofValidationError.t)
+  .
+
+  Global Instance IsLink : Link t := {
+    Φ := Ty.path "revm_bytecode::eof::verification::EofError";
+    φ x :=
+      match x with
+      | Decode γ0 =>
+        Value.StructTuple "revm_bytecode::eof::verification::EofError::Decode" [
+          φ γ0
+        ]
+      | Validation γ0 =>
+        Value.StructTuple "revm_bytecode::eof::verification::EofError::Validation" [
+          φ γ0
+        ]
+      end
+  }.
+End EofError.
+
+Module EofValidationError.
+  Inductive t : Set :=
+  | FalsePositive
+  | UnknownOpcode
+  | OpcodeDisabled
+  | InstructionNotForwardAccessed
+  | MissingImmediateBytes
+  | MissingRJUMPVImmediateBytes
+  | JumpToImmediateBytes
+  | BackwardJumpToImmediateBytes
+  | RJUMPVZeroMaxIndex
+  | JumpZeroOffset
+  | EOFCREATEInvalidIndex
+  | CodeSectionOutOfBounds
+  | CALLFNonReturningFunction
+  | StackOverflow
+  | JUMPFEnoughOutputs
+  | JUMPFStackHigherThanOutputs
+  | DataLoadOutOfBounds
+  | RETFBiggestStackNumMoreThenOutputs
+  | StackUnderflow
+  | TypesStackUnderflow
+  | JumpUnderflow
+  | JumpOverflow
+  | BackwardJumpBiggestNumMismatch
+  | BackwardJumpSmallestNumMismatch
+  | LastInstructionNotTerminating
+  | CodeSectionNotAccessed
+  | InvalidTypesSection
+  | InvalidFirstTypesSection
+  | MaxStackMismatch
+  | NoCodeSections
+  | SubContainerCalledInTwoModes
+  | SubContainerNotAccessed
+  | DataNotFilled
+  | NonReturningSectionIsReturning
+  .
+
+  Global Instance IsLink : Link t := {
+    Φ := Ty.path "revm_bytecode::eof::verification::EofValidationError";
+    φ x :=
+      match x with
+      | FalsePositive  =>
+        Value.StructTuple "revm_bytecode::eof::verification::EofValidationError::FalsePositive" []
+      | UnknownOpcode  =>
+        Value.StructTuple "revm_bytecode::eof::verification::EofValidationError::UnknownOpcode" []
+      | OpcodeDisabled  =>
+        Value.StructTuple "revm_bytecode::eof::verification::EofValidationError::OpcodeDisabled" []
+      | InstructionNotForwardAccessed  =>
+        Value.StructTuple "revm_bytecode::eof::verification::EofValidationError::InstructionNotForwardAccessed" []
+      | MissingImmediateBytes  =>
+        Value.StructTuple "revm_bytecode::eof::verification::EofValidationError::MissingImmediateBytes" []
+      | MissingRJUMPVImmediateBytes  =>
+        Value.StructTuple "revm_bytecode::eof::verification::EofValidationError::MissingRJUMPVImmediateBytes" []
+      | JumpToImmediateBytes  =>
+        Value.StructTuple "revm_bytecode::eof::verification::EofValidationError::JumpToImmediateBytes" []
+      | BackwardJumpToImmediateBytes  =>
+        Value.StructTuple "revm_bytecode::eof::verification::EofValidationError::BackwardJumpToImmediateBytes" []
+      | RJUMPVZeroMaxIndex  =>
+        Value.StructTuple "revm_bytecode::eof::verification::EofValidationError::RJUMPVZeroMaxIndex" []
+      | JumpZeroOffset  =>
+        Value.StructTuple "revm_bytecode::eof::verification::EofValidationError::JumpZeroOffset" []
+      | EOFCREATEInvalidIndex  =>
+        Value.StructTuple "revm_bytecode::eof::verification::EofValidationError::EOFCREATEInvalidIndex" []
+      | CodeSectionOutOfBounds  =>
+        Value.StructTuple "revm_bytecode::eof::verification::EofValidationError::CodeSectionOutOfBounds" []
+      | CALLFNonReturningFunction  =>
+        Value.StructTuple "revm_bytecode::eof::verification::EofValidationError::CALLFNonReturningFunction" []
+      | StackOverflow  =>
+        Value.StructTuple "revm_bytecode::eof::verification::EofValidationError::StackOverflow" []
+      | JUMPFEnoughOutputs  =>
+        Value.StructTuple "revm_bytecode::eof::verification::EofValidationError::JUMPFEnoughOutputs" []
+      | JUMPFStackHigherThanOutputs  =>
+        Value.StructTuple "revm_bytecode::eof::verification::EofValidationError::JUMPFStackHigherThanOutputs" []
+      | DataLoadOutOfBounds  =>
+        Value.StructTuple "revm_bytecode::eof::verification::EofValidationError::DataLoadOutOfBounds" []
+      | RETFBiggestStackNumMoreThenOutputs  =>
+        Value.StructTuple "revm_bytecode::eof::verification::EofValidationError::RETFBiggestStackNumMoreThenOutputs" []
+      | StackUnderflow  =>
+        Value.StructTuple "revm_bytecode::eof::verification::EofValidationError::StackUnderflow" []
+      | TypesStackUnderflow  =>
+        Value.StructTuple "revm_bytecode::eof::verification::EofValidationError::TypesStackUnderflow" []
+      | JumpUnderflow  =>
+        Value.StructTuple "revm_bytecode::eof::verification::EofValidationError::JumpUnderflow" []
+      | JumpOverflow  =>
+        Value.StructTuple "revm_bytecode::eof::verification::EofValidationError::JumpOverflow" []
+      | BackwardJumpBiggestNumMismatch  =>
+        Value.StructTuple "revm_bytecode::eof::verification::EofValidationError::BackwardJumpBiggestNumMismatch" []
+      | BackwardJumpSmallestNumMismatch  =>
+        Value.StructTuple "revm_bytecode::eof::verification::EofValidationError::BackwardJumpSmallestNumMismatch" []
+      | LastInstructionNotTerminating  =>
+        Value.StructTuple "revm_bytecode::eof::verification::EofValidationError::LastInstructionNotTerminating" []
+      | CodeSectionNotAccessed  =>
+        Value.StructTuple "revm_bytecode::eof::verification::EofValidationError::CodeSectionNotAccessed" []
+      | InvalidTypesSection  =>
+        Value.StructTuple "revm_bytecode::eof::verification::EofValidationError::InvalidTypesSection" []
+      | InvalidFirstTypesSection  =>
+        Value.StructTuple "revm_bytecode::eof::verification::EofValidationError::InvalidFirstTypesSection" []
+      | MaxStackMismatch  =>
+        Value.StructTuple "revm_bytecode::eof::verification::EofValidationError::MaxStackMismatch" []
+      | NoCodeSections  =>
+        Value.StructTuple "revm_bytecode::eof::verification::EofValidationError::NoCodeSections" []
+      | SubContainerCalledInTwoModes  =>
+        Value.StructTuple "revm_bytecode::eof::verification::EofValidationError::SubContainerCalledInTwoModes" []
+      | SubContainerNotAccessed  =>
+        Value.StructTuple "revm_bytecode::eof::verification::EofValidationError::SubContainerNotAccessed" []
+      | DataNotFilled  =>
+        Value.StructTuple "revm_bytecode::eof::verification::EofValidationError::DataNotFilled" []
+      | NonReturningSectionIsReturning  =>
+        Value.StructTuple "revm_bytecode::eof::verification::EofValidationError::NonReturningSectionIsReturning" []
+      end
+  }.
+End EofValidationError.
+
+Module AccessTracker.
+  Record t : Set := {
+    this_container_code_type: core.links.option.Option.t revm_bytecode.eof.links.verification.CodeType.t;
+    codes: alloc.links.vec.Vec.t bool alloc.links.alloc.Global.t;
+    processing_stack: alloc.links.vec.Vec.t Usize.t alloc.links.alloc.Global.t;
+    subcontainers: alloc.links.vec.Vec.t (core.links.option.Option.t revm_bytecode.eof.links.verification.CodeType.t) alloc.links.alloc.Global.t;
+  }.
+
+  Global Instance IsLink : Link t := {
+    Φ := Ty.path "revm_bytecode::eof::verification::AccessTracker";
+    φ '(Build_t this_container_code_type codes processing_stack subcontainers) :=
+      Value.StructRecord "revm_bytecode::eof::verification::AccessTracker" [
+        ("this_container_code_type", φ this_container_code_type);
+        ("codes", φ codes);
+        ("processing_stack", φ processing_stack);
+        ("subcontainers", φ subcontainers)
+      ]
+  }.
+End AccessTracker.
+
+Module CodeType.
+  Inductive t : Set :=
+  | ReturnContract
+  | ReturnOrStop
+  .
+
+  Global Instance IsLink : Link t := {
+    Φ := Ty.path "revm_bytecode::eof::verification::CodeType";
+    φ x :=
+      match x with
+      | ReturnContract  =>
+        Value.StructTuple "revm_bytecode::eof::verification::CodeType::ReturnContract" []
+      | ReturnOrStop  =>
+        Value.StructTuple "revm_bytecode::eof::verification::CodeType::ReturnOrStop" []
+      end
+  }.
+End CodeType.
+
+Module InstructionInfo.
+  Record t : Set := {
+    is_immediate: bool;
+    is_jumpdest: bool;
+    smallest: I32.t;
+    biggest: I32.t;
+  }.
+
+  Global Instance IsLink : Link t := {
+    Φ := Ty.path "revm_bytecode::eof::verification::validate_eof_code::InstructionInfo";
+    φ '(Build_t is_immediate is_jumpdest smallest biggest) :=
+      Value.StructRecord "revm_bytecode::eof::verification::validate_eof_code::InstructionInfo" [
+        ("is_immediate", φ is_immediate);
+        ("is_jumpdest", φ is_jumpdest);
+        ("smallest", φ smallest);
+        ("biggest", φ biggest)
+      ]
+  }.
+End InstructionInfo.
+
+Module TypesSection.
+  Record t : Set := {
+    inputs: U8.t;
+    outputs: U8.t;
+    max_stack_size: U16.t;
+  }.
+
+  Global Instance IsLink : Link t := {
+    Φ := Ty.path "revm_bytecode::eof::types_section::TypesSection";
+    φ '(Build_t inputs outputs max_stack_size) :=
+      Value.StructRecord "revm_bytecode::eof::types_section::TypesSection" [
+        ("inputs", φ inputs);
+        ("outputs", φ outputs);
+        ("max_stack_size", φ max_stack_size)
+      ]
+  }.
+End TypesSection.
